To bytes spec proved correct, draft equiv

proof/crypto_scalarmult/curve25519/amd64/ref4/CorrectnessProof_ToBytes.ec
@@ -34,17 +34,17 @@ module ToBytesSpec = {
     return t;
  }
 
- proc sar_inv_t (t: W64.t) : W64.t = {
+ proc to_0_or_19 (t: W64.t) : W64.t = {
     var _of_, _cf_, _sf_, _2, _zf_ : bool;
-    var tt, tt0, tt1 : W64.t;
+    var _tt, tt0, tt1 : W64.t;
 
-    (_of_, _cf_, _sf_, _2, _zf_, tt) <- SAR_64 t ((of_int 63))%W8;
-    tt0 <- invw tt;
+    (_of_, _cf_, _sf_, _2, _zf_, _tt) <- SAR_64 t ((of_int 63))%W8;
+    tt0 <- invw _tt;
     tt1 <- tt0 `&` (of_int 19)%W64;
     return tt1;
  }
 
- proc to19(t: W64.t) : W64.t = {
+ proc to_19_or_38(t: W64.t) : W64.t = {
 
     t <- t `&` (of_int 19)%W64;
     t <- t + (of_int 19)%W64;
@@ -52,11 +52,10 @@ module ToBytesSpec = {
     return t;
  }
 
- proc addition(f: Rep4, operand2: W64.t) : Rep4 = {
-  var aux_4, tt, tt0 : W64.t;
+ proc addition(f: Rep4, _tt: W64.t, operand2: W64.t) : Rep4 = {
+  var aux_4, tt0 : W64.t;
   var _of_, _cf_, _sf_, _zf_, cf, _0, _1, _2, aux_3 : bool;
   var ff : Rep4; (* we don't change the value of f, easier proofs *)
-  tt <- f.[3];
 
   (aux_3, aux_4) <- addc f.[0] operand2 false;
   cf <- aux_3;
@@ -67,7 +66,7 @@ module ToBytesSpec = {
   (aux_3, aux_4) <- addc f.[2] W64.zero cf;
   cf <- aux_3;
   ff <- ff.[2 <- aux_4];
-  (_1, tt0) <- addc tt W64.zero cf;
+  (_1, tt0) <- addc _tt W64.zero cf;
   ff <- ff.[3 <- tt0];
 
   return ff;
@@ -95,34 +94,26 @@ module ToBytesSpec = {
   return ff;
  }
 
- (* We show that for 0 <= valrep4 f < 2^255, the first three calls essentially do nothing *)
- proc addition_calls(f: Rep4) : Rep4 = {
-   var tt, tt0, extracted_msbw : W64.t;
-   var ff : Rep4; (* we don't change the value of f, easier proofs *)
-   ff <- witness;
-   extracted_msbw <@ extract_msb (f.[3]);
-   tt  <@ remove_msb_if_set (f.[3]);
-   tt0 <@ to19 (extracted_msbw);
-   ff <@ addition(f, tt0);
-   return ff;
+
+ proc to_bytes(f: Rep4) : Rep4 = {
+     var msb1, _tt, _tt0, msb2, _f3, _tt2  : W64.t;
+     var ff, ff2, ff3 : Rep4; (* we don't change the value of f, easier proofs *)
+
+     msb1 <@ extract_msb (f.[3]);
+     _tt  <@ remove_msb_if_set (f.[3]);
+     _tt0 <@ to_19_or_38 (msb1);
+     ff   <@ addition(f, _tt, _tt0);
+     _f3  <@ remove_msb_if_set (ff.[3]);
+     ff2 <- ff.[3 <- _f3];
+     _tt2 <@ to_0_or_19(ff.[3]);
+     ff3  <@ subtraction(ff2, _tt2);
+     return ff3;
  }
-
- proc tobytes_no_reduction(f: Rep4) : Rep4 = {
-     var tt, tt0, f3, extracted_msbw : W64.t;
-     var ff, ff2: Rep4; (* we don't change the value of f, easier proofs *)
-
-     ff <@ addition_calls(f);              (* ff = f + 19 *)
-     f3 <@ sar_inv_t(ff.[3]);              (* f3 = 19 *)
-     ff2  <@ subtraction(ff, f3);          (* ff2 = ff - 19 = f + 19 - 19 = f *)
-     return ff2;
- }
-
-
 }.
 
 (* Helper lemmas *)
 lemma cminusP0 r: 0 <= r < p => r = asint (inzp r).
-proof. move => H. rewrite inzpK pE => />. rewrite modz_small. apply bound_abs. smt(pVal). auto. qed.
+proof. move => H. rewrite inzpK pE => />. by rewrite pmod_small; 1:smt(pVal). qed.
 
 lemma cminusP1 r: p <= r < 2*p => r - p = asint (inzp r).
 proof. rewrite inzpK => />. move => [#] H H0. smt(pE pVal). qed.
@@ -130,44 +121,46 @@ proof. rewrite inzpK => />. move => [#] H H0. smt(pE pVal). qed.
 lemma cminusP2 r: 2*p <= r < W256.modulus => r - p - p = asint (inzp r).
 proof. rewrite inzpK => />. move => [#] H H0. smt(pE pVal). qed.
 
-lemma upper_limb4_lt_2_255_range r: 0 <= valRep4 r < pow 2 255 => 0 <= (to_uint r.[3]) < pow 2 63.
-proof. rewrite valRep4E /to_list /val_digits /mkseq -iotaredE => />. smt(W64.to_uint_cmp). qed.
+(** Range lemmas **)
+lemma valRep4_cmp f: 0 <= valRep4 f < W256.modulus.
+proof. rewrite valRep4E /to_list /val_digits /mkseq -iotaredE => />. move: W64.to_uint_cmp. smt(). qed.
 
-lemma upper_limb4_ltP_range r: 0 <= valRep4 r < p => 0 <= (to_uint r.[3]) < pow 2 63.
+lemma limb4_ltP_cmp r: 0 <= valRep4 r < p => 0 <= (to_uint r.[3]) < pow 2 63.
 proof. rewrite valRep4E pE /to_list /val_digits /mkseq -iotaredE => />. smt(W64.to_uint_cmp). qed.
 
-lemma upper_limb4_ltP_msb r: 0 <= valRep4 r < p => r.[3].[63] = false.
-proof. move => H. have E: b2i r.[3].[63] = 0.
-       rewrite b2i_get //=. move: upper_limb4_ltP_range W64.to_uint_cmp; 1:smt(). smt(). qed.
+lemma limb4_lt_2_255_cmp r: 0 <= valRep4 r < pow 2 255 => 0 <= (to_uint r.[3]) < pow 2 63.
+proof. rewrite valRep4E /to_list /val_digits /mkseq -iotaredE => />. smt(W64.to_uint_cmp). qed.
 
-lemma upper_limb4_ltP_msbw r: 0 <=  W64.to_uint r < pow 2 63 => r.[63] = false.
-proof. move => H. have E: b2i r.[63] = 0.
-       rewrite b2i_get //=. move: H. smt(). smt(). qed.
+lemma limb4_gtP_cmp r: p < valRep4 r < W64.modulus => pow 2 63 <= (to_uint r.[3]) < W64.modulus.
+proof. rewrite valRep4E pE /to_list /val_digits /mkseq -iotaredE => />. smt(W64.to_uint_cmp). qed.
 
-lemma upper_limb4_geq_2_255_range r: pow 2 255 <= valRep4 r < W256.modulus =>
+lemma limb4_geq_2_255_cmp r: pow 2 255 <= valRep4 r < W256.modulus =>
            pow 2 63 <= (to_uint r.[3]) < W64.modulus.
 proof. rewrite valRep4E /to_list /val_digits /mkseq -iotaredE => />.
        move => H H0. do split. move: W64.to_uint_cmp. smt(). move: W64.to_uint_cmp. smt(). qed.
 
-lemma upper_limb4_p_2_255_range r: p <= valRep4 r < pow 2 255 =>
-           pow 2 63 - 1 <= (to_uint r.[3]) < W64.modulus.
-proof. rewrite valRep4E pE /to_list /val_digits /mkseq -iotaredE => />.
-       move => H H0. do split. move: W64.to_uint_cmp. smt(). move: W64.to_uint_cmp. smt(). qed.
+(** MSB lemmas **)
+lemma limb4_msbw0 r: 0 <=  W64.to_uint r < pow 2 63 => r.[63] = false.
+proof. move => H. have E: b2i r.[63] = 0.
+       rewrite b2i_get //=. move: H. smt(). smt(). qed.
 
-lemma upper_limb4_geqP_range r: p <= valRep4 r < W256.modulus =>
-           (pow 2 63) - 1 <= (to_uint r.[3]) < W64.modulus.
-proof. rewrite valRep4E pE /to_list /val_digits /mkseq -iotaredE => />.
-       move => H H0. do split. move: W64.to_uint_cmp. smt(). move: W64.to_uint_cmp. smt(). qed.
-
-lemma upper_limb4_geq_2_255_msb r: pow 2 255 <= valRep4 r < W256.modulus => r.[3].[63] = true.
-proof. move => H. have E: b2i r.[3].[63] = 1.
-       rewrite b2i_get //=. move: H upper_limb4_geq_2_255_range W64.to_uint_cmp; 1:smt(). smt(). qed.
-
-lemma upper_limb4_geqP_msbw r: pow 2 63  <=  W64.to_uint r < W64.modulus => r.[63] = true.
+lemma limb4_msbw1 r: pow 2 63 <= W64.to_uint r < W64.modulus => r.[63] = true.
 proof. move => H. have E: b2i r.[63] = 1.
-       rewrite b2i_get //=. move: H upper_limb4_geq_2_255_range W64.to_uint_cmp; 1:smt(). smt(). qed.
+       rewrite b2i_get //=. move: H. smt(). smt(). qed.
 
-lemma helper_remove_msb_if_set (f: W64.t):
+lemma limb4_ltP_msb r: 0 <= valRep4 r < p => r.[3].[63] = false.
+proof. move => H. have E: b2i r.[3].[63] = 0.
+       rewrite b2i_get //=. move: limb4_ltP_cmp W64.to_uint_cmp; 1:smt(). smt(). qed.
+
+lemma limb4_gtP_msb r: p < valRep4 r < W64.modulus => r.[3].[63] = true.
+proof. move => H. have E: b2i r.[3].[63] = 1.
+       rewrite b2i_get //=. move: H.
+       rewrite valRep4E pE /to_list /val_digits /mkseq -iotaredE => />. smt(W64.to_uint_cmp).
+       smt().
+qed.
+
+(** Helper lemmas **)
+lemma helper_lemma_msb_is_not_set (f: W64.t):
     0 <= W64.to_uint f < pow 2 63 => LEA_64 (f + f) `>>` W8.one = f.
 proof.
     auto => />. rewrite /LEA_64 => *.
@@ -176,13 +169,46 @@ proof.
     smt(). smt(). smt(@W64).
 qed.
 
-lemma helper_sar_inv_t (t: W64.t) : 0 <= u64i t && u64i t < pow 2 63 => invw (SAR_64 t ((of_int 63))%W8).`6 `&` (of_int 19)%W64 = (of_int 19)%W64.
+lemma helper_lemma_extract_msb_0 (f: W64.t) : 0 <= W64.to_uint f < pow 2 63 => (SAR_64 f ((of_int 63))%W8).`6 = W64.zerow.
+proof.
+    auto => />. move => H H0. rewrite /SAR_64 /shift_mask /rflags_OF //= sarE.
+    rewrite init_bits2w bits2wE -iotaredE /min //=.
+    rewrite limb4_msbw0 //=.
+    + rewrite /W64.zerow /W64.zero bits2wE /int2bs /mkseq -iotaredE => />.
+qed.
+
+lemma helper_lemma_extract_msb_1 (f: W64.t) : pow 2 63 <= W64.to_uint f < pow 2 64 => (SAR_64 f ((of_int 63))%W8).`6 = W64.onew.
+proof.
+    auto => />. move => H H0. rewrite /SAR_64 /shift_mask /rflags_OF //= sarE.
+    rewrite init_bits2w bits2wE -iotaredE /min //=.
+    rewrite limb4_msbw1 //=.
+    + rewrite /W64.onew of_intE  bits2wE /int2bs /mkseq -iotaredE => />.
+qed.
+
+lemma helper_lemma_remove_msb (f: W64.t):
+    pow 2 63 <= W64.to_uint f < pow 2 64 => LEA_64 (f + f) `>>` W8.one = f - W64.of_int (pow 2 63).
+proof.
+    auto => />. rewrite /LEA_64 => *.
+    rewrite shr_shrw //= addE !/ulift2 of_intE => />. rewrite of_intE.
+    have !->: (u64i f + u64i f) %% 18446744073709551616 = (u64i f + u64i f) - 18446744073709551616. smt().
+    rewrite !to_uintN !of_uintK.
+    have !->: - 9223372036854775808 %% pow 2 64 =
+                9223372036854775808 - pow 2 64. smt(). auto => />.
+    have !->: (u64i f + 9223372036854775808) %% 18446744073709551616 =
+              (u64i f + 9223372036854775808) - 18446744073709551616.
+    move: W64.to_uint_cmp. smt(). auto => />.
+    rewrite wlsrE init_bits2w. congr. rewrite /int2bs /mkseq -!iotaredE => />.
+    do split; 1..63:smt().
+    rewrite get_out /#.
+qed.
+
+lemma helper_lemma_to_19 (t: W64.t) : 0 <= u64i t && u64i t < pow 2 63 => invw (SAR_64 t ((of_int 63))%W8).`6 `&` (of_int 19)%W64 = (of_int 19)%W64.
 proof.
     auto => />. move => H H0.
     have ->: (SAR_64 t ((of_int 63))%W8).`6 = W64.zerow.
     + rewrite /SAR_64 /shift_mask /rflags_OF //= sarE /min => />.
     rewrite init_bits2w bits2wE -iotaredE /min //=.
-    rewrite upper_limb4_ltP_msbw //=.
+    rewrite limb4_msbw0 //=.
     + rewrite /W64.zerow /W64.zero bits2wE /int2bs /mkseq -iotaredE => />.
     have ->: invw W64.zerow = W64.onew.
     + rewrite /invw mapE /W64.zerow /W64.zero bits2wE /int2bs /mkseq -iotaredE => />.
@@ -193,119 +219,487 @@ proof.
     rewrite !initiE 1,2:/# //= /#.
 qed.
 
+lemma helper_lemma_to_0 (t: W64.t) : pow 2 63 <= u64i t && u64i t < pow 2 64 => invw (SAR_64 t ((of_int 63))%W8).`6 `&` (of_int 19)%W64 = (of_int 0)%W64.
+proof.
+    auto => />. move => H H0.
+    have ->: (SAR_64 t ((of_int 63))%W8).`6 = W64.onew.
+    + rewrite /SAR_64 /shift_mask /rflags_OF //= sarE /min => />.
+    rewrite init_bits2w bits2wE -iotaredE /min //=.
+    rewrite limb4_msbw1 //=.
+    + rewrite /W64.onew of_intE bits2wE /int2bs /mkseq -iotaredE => />.
+    have ->: invw W64.onew = W64.zerow.
+    + rewrite /invw mapE /W64.zerow /W64.zero bits2wE /int2bs /mkseq -iotaredE => />.
+    + rewrite wordP => i ib. rewrite !initiE 1,2:/# //=. smt().
+    rewrite wordP => i ib.
+    rewrite /W64.onew !of_intE !bits2wE !/int2bs !/mkseq -!iotaredE => />.
+    rewrite !initiE 1,2:/# //= /#.
+qed.
+
 lemma not_false_to_true bst: (bst <> false) = (bst = true) by smt().
+
+lemma valRep4_equiv_representation (r: Rep4): r = (of_list witness [r.[0]; r.[1]; r.[2]; r.[3]])%Array4.
+proof.
+    auto => />. apply Array4.ext_eq => i ib.
+    case (i = 3) => I. rewrite I => />.
+    case (i = 2) => I0. rewrite I0 => />.
+    case (i = 1) => I1. rewrite I1 => />.
+    case (i = 0) => I2. rewrite I2 => />. rewrite get_out /#.
+qed.
+
+lemma valRep4_remove_limb4_ltP r: 0 <= valRep4 r < p => valRep4 r.[3 <- W64.zerow] < p - u64i r.[3].
+proof.
+    auto => />.
+    rewrite !valRep4E !pE !/to_list !/val_digits !/mkseq -!iotaredE => />.
+    rewrite to_uint0 => />. smt(W64.to_uint_cmp).
+qed.
+
+lemma valRep4_remove_limb4_geP_lt_2_255 r: p <= valRep4 r < pow 2 255 => valRep4 r.[3 <- W64.zerow] < pow 2 255 - u64i r.[3].
+proof.
+    auto => />.
+    rewrite !valRep4E !pE !/to_list !/val_digits !/mkseq -!iotaredE => />.
+    rewrite to_uint0 => />. smt(W64.to_uint_cmp).
+qed.
+
+lemma valRep4_remove_limb4_ltP_structure r: 0 <= valRep4 r < p => r.[3 <- W64.zerow] = (of_list witness [r.[0]; r.[1]; r.[2]; W64.zerow])%Array4.
+proof.
+    auto => />. move => H H0. apply Array4.ext_eq => i ib.
+    rewrite !get_setE 1:/#.
+    case (i = 3) => I. rewrite I => />.
+    case (i = 2) => I0. rewrite I0 => />.
+    case (i = 1) => I1. rewrite I1 => />.
+    case (i = 0) => I2. rewrite I2 => />. rewrite get_out /#.
+qed.
+
+lemma valRep4_remove_limb4_ltP_structure_2 r: p <= valRep4 r < pow 2 255 => r.[3 <- W64.zerow] = (of_list witness [r.[0]; r.[1]; r.[2]; W64.zerow])%Array4.
+proof.
+    auto => />. move => H H0. apply Array4.ext_eq => i ib.
+    rewrite !get_setE 1:/#.
+    case (i = 3) => I. rewrite I => />.
+    case (i = 2) => I0. rewrite I0 => />.
+    case (i = 1) => I1. rewrite I1 => />.
+    case (i = 0) => I2. rewrite I2 => />. rewrite get_out /#.
+qed.
+
+abbrev add_l1 (r: Rep4, i: int) = (addc r.[0] ((of_int i))%W64 false).`2.
+abbrev add_l2 (r: Rep4, i: int) = (addc r.[1] W64.zero (addc_carry r.[0] ((of_int i))%W64 false)).`2.
+abbrev add_l3 (r: Rep4, i: int) = (addc r.[2] W64.zero (addc_carry r.[1] W64.zero (addc_carry r.[0] ((of_int i))%W64 false))).`2.
+abbrev add_l4 (r: Rep4, __tt: W64.t, i: int) = (addc __tt W64.zero (addc_carry r.[2] W64.zero (addc_carry r.[1] W64.zero (addc_carry r.[0] ((of_int i))%W64 false)))).`2.
+
+abbrev add_to_limb (r: Rep4, __tt: W64.t, i: int) = Array4.of_list witness [add_l1 r i; add_l2 r i; add_l3 r i; add_l4 r __tt i ].
+
+abbrev sub_l1 (r: Rep4, i: int) = (subc r.[0] ((of_int i))%W64 false).`2.
+abbrev sub_l2 (r: Rep4, i: int) = (subc r.[1] W64.zero (subc_borrow r.[0] ((of_int i))%W64 false)).`2.
+abbrev sub_l3 (r: Rep4, i: int) = (subc r.[2] W64.zero (subc_borrow r.[1] W64.zero (subc_borrow r.[0] ((of_int i))%W64 false))).`2.
+abbrev sub_l4 (r: Rep4, i: int) = (subc r.[3] W64.zero (subc_borrow r.[2] W64.zero (subc_borrow r.[1] W64.zero (subc_borrow r.[0] ((of_int i))%W64 false)))).`2.
+
+abbrev sub_from_limb (r: Rep4, i: int) = Array4.of_list witness [sub_l1 r i; sub_l2 r i; sub_l3 r i; sub_l4 r i ].
+
+lemma limb4_valRep4_add19_cmp f __tt: valRep4 (add_to_limb f __tt 19) < p + 19 => 0 <= u64i (add_l4 f __tt 19) => u64i (add_l4 f __tt 19) < 9223372036854775808.
+proof.
+   + rewrite !valRep4E !pVal !/to_list !/val_digits !/mkseq -!iotaredE => />.
+   + rewrite !addcE !/carry_add !b2i0 => />.
+   + case (18446744073709551616 <= u64i f.[0] + 19 = false) => C. rewrite !C !b2i0 => />.
+   + have !->: 18446744073709551616 <= u64i f.[1] = false. move: W64.to_uint_cmp. smt().
+   + have !->: 18446744073709551616 <= u64i f.[2] = false. move: W64.to_uint_cmp. smt().
+   + rewrite !b2i0 => />. smt(W64.to_uint_cmp).
+   + move: C. rewrite not_false_to_true. move => C. rewrite !C !b2i1 => />.
+   + case (18446744073709551616 <= u64i f.[1] + 1 = false) => C1. rewrite !C1 !b2i0 => />.
+   + have !->: 18446744073709551616 <= u64i f.[2] = false. move: W64.to_uint_cmp. smt().
+   + rewrite !b2i0 => />. smt(W64.to_uint_cmp).
+   + move: C1. rewrite not_false_to_true. move => C1. rewrite !C1 !b2i1 => />.
+   + case (18446744073709551616 <= u64i f.[2] + 1 = false) => C2. rewrite !C2 !b2i0 => />.
+   + smt(W64.to_uint_cmp).
+   + move: C2. rewrite not_false_to_true. move => C2. rewrite !C2 !b2i1 => />.
+   + rewrite !to_uintD of_uintK. smt(W64.to_uint_cmp).
+qed.
+
+lemma limb4_add19_range_l4_ltP r __tt: 0 <= valRep4 r =>
+  valRep4 r < p =>
+  valRep4 r + 19 = valRep4 (add_to_limb r __tt 19) =>
+  0 <= u64i (add_l4 r __tt 19) /\
+  (0 <= u64i (add_l4 r __tt 19) => u64i (add_l4 r __tt 19) < 9223372036854775808).
+proof.
+    rewrite !addcE !/add_carry !/carry_add !b2i0 => />.
+    rewrite !valRep4E !pVal !/to_list !/val_digits !/mkseq -!iotaredE => />.
+    rewrite !mulzDr -!mulzA !to_uintD !of_uintK (modz_small 19 (pow 2 64)) 1:/# => />.
+    move: (limb4_ltP_cmp r) W64.to_uint_cmp. smt().
+qed.
+
+lemma limb4_add_equiv_ltP r:
+0 <= valRep4 r =>
+valRep4 r < p =>
+u64i r.[3] < 18446744073709551597 /\
+(u64i r.[3] < 18446744073709551597 =>
+ valRep4 ((of_list witness [r.[0]; r.[1]; r.[2]; r.[3]]))%Array4 + 19 =
+ valRep4 (add_to_limb r r.[3] 19) =>
+ valRep4 r + 19 = valRep4 (add_to_limb r r.[3] 19)).
+proof.
+  rewrite pVal -valRep4_equiv_representation.
+  rewrite !valRep4E !/to_list !/val_digits !/mkseq -!iotaredE => />. smt(W64.to_uint_cmp).
+qed.
+
+lemma limb4_add_equiv_geqP_lt_2p r:
+p <= valRep4 r =>
+valRep4 r <
+57896044618658097711785492504343953926634992332820282019728792003956564819968 =>
+u64i r.[3] < 18446744073709551597 /\
+(u64i r.[3] < 18446744073709551597 =>
+ valRep4 ((of_list witness [r.[0]; r.[1]; r.[2]; r.[3]]))%Array4 + 19 =
+ valRep4 (add_to_limb r r.[3] 19) =>
+ valRep4 r + 19 = valRep4 (add_to_limb r r.[3] 19)).
+proof.
+  rewrite pVal -valRep4_equiv_representation.
+  rewrite !valRep4E !/to_list !/val_digits !/mkseq -!iotaredE => />. smt(W64.to_uint_cmp).
+qed.
+
+lemma limb4_add_sub_equiv_geq2P r:
+2 * p <= valRep4 r =>
+valRep4 r <
+115792089237316195423570985008687907853269984665640564039457584007913129639936 =>
+u64i (r.[3] - (of_int 9223372036854775808)%W64) =
+u64i r.[3] - 9223372036854775808 =>
+u64i (r.[3] - (of_int 9223372036854775808)%W64) < 18446744073709551578 /\
+(u64i (r.[3] - (of_int 9223372036854775808)%W64) < 18446744073709551578 =>
+ valRep4
+   ((of_list witness
+       [r.[0]; r.[1]; r.[2]; r.[3] - (of_int 9223372036854775808)%W64]))%Array4 +
+ 38 = valRep4 (add_to_limb r (r.[3] - (of_int 9223372036854775808)%W64) 38) =>
+ valRep4 r -
+ 57896044618658097711785492504343953926634992332820282019728792003956564819930 =
+ valRep4 (add_to_limb r (r.[3] - (of_int 9223372036854775808)%W64) 38)).
+proof.
+    rewrite !pVal.
+    move => H H0 H1.
+    do split. rewrite H1. move: W64.to_uint_cmp. smt().
+    move => H2 H3. rewrite -H3.
+    move: H H0 H1 H2 H3. rewrite !valRep4E !/to_list !/val_digits !/mkseq -!iotaredE => />.
+    + move: W64.to_uint_cmp. smt(@W64).
+qed.
+
+lemma limb4_add_sub_equiv_geqP_lt_2p r:
+57896044618658097711785492504343953926634992332820282019728792003956564819968 <=
+valRep4 r =>
+valRep4 r < 2 * p =>
+u64i (r.[3] - (of_int 9223372036854775808)%W64) =
+u64i r.[3] - 9223372036854775808 =>
+u64i (r.[3] - (of_int 9223372036854775808)%W64) < 18446744073709551578 /\
+(u64i (r.[3] - (of_int 9223372036854775808)%W64) < 18446744073709551578 =>
+ valRep4
+   ((of_list witness
+       [r.[0]; r.[1]; r.[2]; r.[3] - (of_int 9223372036854775808)%W64]))%Array4 +
+ 38 = valRep4 (add_to_limb r (r.[3] - (of_int 9223372036854775808)%W64) 38) =>
+ valRep4 r -
+ 57896044618658097711785492504343953926634992332820282019728792003956564819930 =
+ valRep4 (add_to_limb r (r.[3] - (of_int 9223372036854775808)%W64) 38)).
+proof.
+    move: (limb4_geq_2_255_cmp r) W64.to_uint_cmp.
+    rewrite !valRep4E !pVal !/to_list !/val_digits !/mkseq -!iotaredE => />. smt().
+qed.
+
+lemma limb4_add_range_ltP r:
+0 <= valRep4 r =>
+valRep4 r < p =>
+valRep4 r + 19 = valRep4 (add_to_limb r r.[3] 19) =>
+0 <= u64i (add_l4 r r.[3] 19) /\
+(0 <= u64i (add_l4 r r.[3] 19) =>
+ u64i (add_l4 r r.[3] 19) < 9223372036854775808).
+proof.
+    rewrite !addcE !/add_carry !/carry_add !b2i0 => />.
+    rewrite !valRep4E !pVal !/to_list !/val_digits !/mkseq -!iotaredE => />.
+    rewrite !mulzDr -!mulzA !to_uintD !of_uintK (modz_small 19 (pow 2 64)) 1:/# => />.
+    move: W64.to_uint_cmp limb4_gtP_cmp. smt().
+qed.
+
+lemma limb4_add_range_geqP_lt_2_255 r:
+p <= valRep4 r =>
+valRep4 r <
+pow 2 255 =>
+valRep4 r + 19 = valRep4 (add_to_limb r r.[3] 19) =>
+9223372036854775808 <= u64i (add_l4 r r.[3] 19) /\
+(9223372036854775808 <= u64i (add_l4 r r.[3] 19) =>
+ u64i (add_l4 r r.[3] 19) < 18446744073709551616).
+proof.
+    rewrite !addcE !/add_carry !/carry_add !b2i0 => />.
+    rewrite !valRep4E !pVal !/to_list !/val_digits !/mkseq -!iotaredE => />.
+    rewrite !mulzDr -!mulzA !to_uintD !of_uintK (modz_small 19 (pow 2 64)) 1:/# => />.
+    move: W64.to_uint_cmp limb4_gtP_cmp. smt().
+qed.
+
+lemma limb4_add_range_geq_2_255_lt_2p r:
+57896044618658097711785492504343953926634992332820282019728792003956564819968 <=
+valRep4 r =>
+valRep4 r < 2 * p =>
+u64i (r.[3] - (of_int 9223372036854775808)%W64) =
+u64i r.[3] - 9223372036854775808 =>
+valRep4 r -
+57896044618658097711785492504343953926634992332820282019728792003956564819930 =
+valRep4 (add_to_limb r (r.[3] - (of_int 9223372036854775808)%W64) 38) =>
+0 <= u64i (add_l4 r (r.[3] - (of_int 9223372036854775808)%W64) 38) /\
+(0 <= u64i (add_l4 r (r.[3] - (of_int 9223372036854775808)%W64) 38) =>
+ u64i (add_l4 r (r.[3] - (of_int 9223372036854775808)%W64) 38) <
+ 9223372036854775808).
+proof.
+    move => H H0 H1 H2.
+    do split. smt(W64.to_uint_cmp). move => H3. rewrite !addcE !/carry_add !b2i0 => />.
+    + rewrite to_uintD. rewrite !H1.
+    + move: H H0 H1 H2 H3. rewrite !valRep4E !pVal !/to_list !/val_digits !/mkseq -!iotaredE => />.
+    + move: W64.to_uint_cmp. smt(@W64).
+qed.
+
+lemma limb4_add_range_geq2P r:
+2 * p <= valRep4 r =>
+valRep4 r <
+115792089237316195423570985008687907853269984665640564039457584007913129639936 =>
+u64i (r.[3] - (of_int 9223372036854775808)%W64) =
+u64i r.[3] - 9223372036854775808 =>
+valRep4 r -
+57896044618658097711785492504343953926634992332820282019728792003956564819930 =
+valRep4 (add_to_limb r (r.[3] - (of_int 9223372036854775808)%W64) 38) =>
+9223372036854775808 <=
+u64i (add_l4 r (r.[3] - (of_int 9223372036854775808)%W64) 38) /\
+(9223372036854775808 <=
+ u64i (add_l4 r (r.[3] - (of_int 9223372036854775808)%W64) 38) =>
+ u64i (add_l4 r (r.[3] - (of_int 9223372036854775808)%W64) 38) <
+ 18446744073709551616).
+proof.
+    move => H H0 H1 H2.
+    do split. rewrite !addcE !/carry_add !b2i0 => />.
+    rewrite to_uintD. rewrite H1.
+    + move: H H1 H2 pVal W64.to_uint_cmp.
+    + rewrite !valRep4E !pVal !/to_list !/val_digits !/mkseq -!iotaredE => />. smt(@W64).
+    move => H3.
+    + move: H H1 H2 pVal W64.to_uint_cmp.
+    + rewrite !valRep4E !pVal !/to_list !/val_digits !/mkseq -!iotaredE => />. smt(@W64).
+qed.
+
+lemma limb4_set_f3_geq_2_255_lt_2p r:
+p <= valRep4 r =>
+valRep4 r <
+57896044618658097711785492504343953926634992332820282019728792003956564819968 =>
+valRep4 r + 19 = valRep4 (add_to_limb r r.[3] 19) =>
+valRep4
+  (add_to_limb r r.[3] 19).[3 <-
+    add_l4 r r.[3] 19 - (of_int 9223372036854775808)%W64] =
+valRep4 (add_to_limb r r.[3] 19) -
+57896044618658097711785492504343953926634992332820282019728792003956564819968.
+proof.
+    rewrite !addcE !/add_carry !/carry_add !b2i0 => />.
+    rewrite !valRep4E !pVal !/to_list !/val_digits !/mkseq -!iotaredE => />.
+    rewrite !mulzDr -!mulzA !to_uintD !of_uintK (modz_small 19 (pow 2 64)) 1:/# => />.
+    case (18446744073709551616 <= u64i r.[0] + 19 = false) => C. rewrite !C !b2i0 => />.
+   + have !->: 18446744073709551616 <= u64i r.[1] = false. move: W64.to_uint_cmp. smt().
+   + have !->: 18446744073709551616 <= u64i r.[2] = false. move: W64.to_uint_cmp. smt().
+   + rewrite !b2i0 => />. smt(W64.to_uint_cmp).
+   + move: C. rewrite not_false_to_true. move => C. rewrite !C !b2i1 => />.
+   + case (18446744073709551616 <= u64i r.[1] + 1 = false) => C1. rewrite !C1 !b2i0 => />.
+   + have !->: 18446744073709551616 <= u64i r.[2] = false. move: W64.to_uint_cmp. smt().
+   + rewrite !b2i0 => />. smt(W64.to_uint_cmp).
+   + move: C1. rewrite not_false_to_true. move => C1. rewrite !C1 !b2i1 => />.
+   + case (18446744073709551616 <= u64i r.[2] + 1 = false) => C2. rewrite !C2 !b2i0 => />.
+   + smt(W64.to_uint_cmp).
+   + move: C2. rewrite not_false_to_true. move => C2. rewrite !C2 !b2i1 => />.
+   + rewrite !to_uintN. smt().
+qed.
+
+lemma limb4_set_f3_gtP_lt_2p r:
+57896044618658097711785492504343953926634992332820282019728792003956564819968 <=
+valRep4 r =>
+valRep4 r < 2 * p =>
+u64i (r.[3] - (of_int 9223372036854775808)%W64) =
+u64i r.[3] - 9223372036854775808 =>
+valRep4 r -
+57896044618658097711785492504343953926634992332820282019728792003956564819930 =
+valRep4 (add_to_limb r (r.[3] - (of_int 9223372036854775808)%W64) 38) =>
+valRep4
+  (add_to_limb r (r.[3] - (of_int 9223372036854775808)%W64) 38).[3 <-
+    add_l4 r (r.[3] - (of_int 9223372036854775808)%W64) 38] =
+valRep4 (add_to_limb r (r.[3] - (of_int 9223372036854775808)%W64) 38).
+proof.
+    rewrite !addcE !/add_carry !/carry_add !b2i0 => />.
+    rewrite !valRep4E !pVal !/to_list !/val_digits !/mkseq -!iotaredE => />.
+qed.
+
+lemma limb4_set_f3_gt2P r:
+2 * p <= valRep4 r =>
+valRep4 r <
+115792089237316195423570985008687907853269984665640564039457584007913129639936 =>
+u64i (r.[3] - (of_int 9223372036854775808)%W64) =
+u64i r.[3] - 9223372036854775808 =>
+valRep4 r -
+57896044618658097711785492504343953926634992332820282019728792003956564819930 =
+valRep4 (add_to_limb r (r.[3] - (of_int 9223372036854775808)%W64) 38) =>
+valRep4
+  (add_to_limb r (r.[3] - (of_int 9223372036854775808)%W64) 38).[3 <-
+    add_l4 r (r.[3] - (of_int 9223372036854775808)%W64) 38 -
+    (of_int 9223372036854775808)%W64] =
+valRep4 (add_to_limb r (r.[3] - (of_int 9223372036854775808)%W64) 38) -
+57896044618658097711785492504343953926634992332820282019728792003956564819968.
+proof.
+    move => H H0 H1 H2. rewrite -H2 => />.
+    move: H H0 H1 H2.
+    rewrite !addcE !/add_carry !/carry_add !b2i0 => />.
+    rewrite !valRep4E !pVal !/to_list !/val_digits !/mkseq -!iotaredE => />.
+    move: W64.to_uint_cmp. smt(@W64).
+qed.
+
+lemma limb4_minus_2_63_equiv r:
+57896044618658097711785492504343953926634992332820282019728792003956564819968 <=
+valRep4 r =>
+valRep4 r < 2 * p =>
+u64i (r.[3] - (of_int (pow 2 63))%W64) = u64i r.[3] - 9223372036854775808.
+proof.
+move: (limb4_geq_2_255_cmp r) W64.to_uint_cmp.
+rewrite !valRep4E !pVal !/to_list !/val_digits !/mkseq -!iotaredE => />. smt(@W64).
+qed.
+
+lemma limb4_minus_2_63_add38_equiv (r: Rep4):
+57896044618658097711785492504343953926634992332820282019728792003956564819968 <=
+valRep4 r =>
+valRep4 r < 2 * p =>
+u64i (r.[3] - (of_int 9223372036854775808)%W64) =
+u64i r.[3] - 9223372036854775808 =>
+valRep4 r -
+57896044618658097711785492504343953926634992332820282019728792003956564819930 =
+valRep4 (add_to_limb r (r.[3] - (of_int 9223372036854775808)%W64) 38) =>
+LEA_64
+  (add_l4 r (r.[3] - (of_int 9223372036854775808)%W64) 38 +
+   add_l4 r (r.[3] - (of_int 9223372036854775808)%W64) 38) `>>`
+W8.one = add_l4 r (r.[3] - (of_int 9223372036854775808)%W64) 38.
+proof.
+    move => H H0 H1 H2. rewrite helper_lemma_msb_is_not_set.
+    do split. move: W64.to_uint_cmp. smt(). move => H3.
+    + rewrite !addcE !/carry_add !b2i0 => />.
+    + rewrite to_uintD. rewrite !H1.
+    + move: H H0 H1 H2 H3. rewrite !valRep4E !pVal !/to_list !/val_digits !/mkseq -!iotaredE => />.
+    + move: W64.to_uint_cmp. smt(@W64). auto.
+qed.
+
+lemma limb4_minus_2_63_add38_equiv_2 (r: Rep4):
+2 * p <= valRep4 r =>
+valRep4 r <
+115792089237316195423570985008687907853269984665640564039457584007913129639936 =>
+u64i (r.[3] - (of_int 9223372036854775808)%W64) =
+u64i r.[3] - 9223372036854775808 =>
+valRep4 r -
+57896044618658097711785492504343953926634992332820282019728792003956564819930 =
+valRep4 (add_to_limb r (r.[3] - (of_int 9223372036854775808)%W64) 38) =>
+LEA_64
+  (add_l4 r (r.[3] - (of_int 9223372036854775808)%W64) 38 +
+   add_l4 r (r.[3] - (of_int 9223372036854775808)%W64) 38) `>>`
+W8.one =
+add_l4 r (r.[3] - (of_int 9223372036854775808)%W64) 38 -
+(of_int 9223372036854775808)%W64.
+proof.
+    move => H H0 H1 H2. rewrite helper_lemma_remove_msb.
+    + rewrite !addcE !/carry_add !b2i0 => />.
+    + rewrite to_uintD. rewrite !H1.
+    + move: H H0 H1 H2. rewrite !valRep4E !pVal !/to_list !/val_digits !/mkseq -!iotaredE => />.
+    + move: W64.to_uint_cmp. smt(@W64). auto.
+qed.
+
+
+lemma limb4_minus_2_63_equiv_2 r:
+2 * p <= valRep4 r =>
+valRep4 r <
+115792089237316195423570985008687907853269984665640564039457584007913129639936 =>
+u64i (r.[3] - (of_int (pow 2 63))%W64) = u64i r.[3] - 9223372036854775808.
+proof.
+move: (limb4_geq_2_255_cmp r) W64.to_uint_cmp.
+rewrite !valRep4E !pVal !/to_list !/val_digits !/mkseq -!iotaredE => />. smt(@W64).
+qed.
 
 
 (** Lossless lemmas **)
-
-lemma ill_sar_inv_t: islossless ToBytesSpec.sar_inv_t by proc; wp; skip => />.
-lemma ill_remove_msb_if_set_lt_2_255: islossless ToBytesSpec.remove_msb_if_set by proc; wp; skip => />.
-lemma ill_extract_msb_lt_2_255: islossless ToBytesSpec.extract_msb by proc; wp; skip => />.
-lemma ill_to19: islossless ToBytesSpec.to19 by proc; wp; skip => />.
+lemma ill_to_0_or_19: islossless ToBytesSpec.to_0_or_19 by proc; wp; skip => />.
+lemma ill_remove_msb_if_set: islossless ToBytesSpec.remove_msb_if_set by proc; wp; skip => />.
+lemma ill_extract_msb: islossless ToBytesSpec.extract_msb by proc; wp; skip => />.
+lemma ill_to_19_or_38: islossless ToBytesSpec.to_19_or_38 by proc; wp; skip => />.
 lemma ill_addition: islossless ToBytesSpec.addition by proc; wp; skip => />.
 lemma ill_subtraction: islossless ToBytesSpec.subtraction by proc; wp; skip => />.
+lemma ill_tobytes: islossless ToBytesSpec.to_bytes by proc; inline *; wp; skip => />.
 
-(** Case: 0 <= valRep4 f < p (some lemmas can be till < 2 255) **)
+(** Word to 19 or 0 by using invw **)
+lemma h_to_19_by_invw:
+  hoare [ToBytesSpec.to_0_or_19 :
+  0 <= W64.to_uint t < pow 2 63 ==> res = W64.of_int 19].
+proof. proc => />. auto => />. move => &h H H0. rewrite helper_lemma_to_19. smt(). auto. qed.
 
-(** SAR+INV+AND **)
-lemma h_sar_inv_t:
-  hoare [ToBytesSpec.sar_inv_t :
-      0 <= W64.to_uint t < pow 2 63
-      ==>
-      res = W64.of_int 19].
-    proc => />. auto => />.
-    move => &h H H0. rewrite helper_sar_inv_t. smt(). auto.
-qed.
+lemma ph_to_19_by_invw:
+  phoare [ToBytesSpec.to_0_or_19 : 0 <= W64.to_uint t < pow 2 63 ==> res = W64.of_int 19] = 1%r.
+proof. by conseq ill_to_0_or_19 (h_to_19_by_invw). qed.
 
-lemma ph_sar_inv_t:
-  phoare [ToBytesSpec.sar_inv_t :
-      0 <= W64.to_uint t < pow 2 63
-      ==>
-      res = W64.of_int 19] = 1%r.
-proof.
-    by conseq ill_sar_inv_t (h_sar_inv_t).
-qed.
+lemma h_to_0_by_invw:
+  hoare [ToBytesSpec.to_0_or_19 :
+      pow 2 63  <= W64.to_uint t < pow 2 64 ==> res = W64.of_int 0].
+proof. proc => />. auto => />. move => &h H H0. rewrite helper_lemma_to_0. smt(). auto. qed.
+
+lemma ph_to_0_by_invw:
+  phoare [ToBytesSpec.to_0_or_19 : pow 2 63  <= W64.to_uint t < pow 2 64 ==> res = W64.of_int 0] = 1%r.
+proof. by conseq ill_to_0_or_19 (h_to_0_by_invw). qed.
 
 (** Remove MSB if it is set **)
-lemma h_remove_msb_if_set_lt_2_255 (r: W64.t):
-  hoare [ToBytesSpec.remove_msb_if_set :
-      r = f3 /\ 0 <= W64.to_uint r < pow 2 63
-      ==>
-      r = res
-  ].
-    proc => />. wp; skip => />. move => *.
-    rewrite helper_remove_msb_if_set /#.
-qed.
+lemma h_msb_not_set (r: W64.t):
+  hoare [ToBytesSpec.remove_msb_if_set : r = f3 /\ 0 <= W64.to_uint r < pow 2 63 ==> r = res].
+proof. proc => />. wp; skip => />. move => *. rewrite helper_lemma_msb_is_not_set /#. qed.
 
-lemma ph_remove_msb_if_set_lt_2_255 (r: W64.t):
-  phoare [ToBytesSpec.remove_msb_if_set :
-      r = f3 /\ 0 <= W64.to_uint r < pow 2 63
-      ==>
-      r = res] = 1%r.
-proof.
-    by conseq ill_remove_msb_if_set_lt_2_255 (h_remove_msb_if_set_lt_2_255 r).
-qed.
+lemma ph_msb_not_set (r: W64.t):
+  phoare [ToBytesSpec.remove_msb_if_set : r = f3 /\ 0 <= W64.to_uint r < pow 2 63 ==> r = res] = 1%r.
+proof. by conseq ill_remove_msb_if_set (h_msb_not_set r). qed.
+
+lemma h_remove_msb (r: W64.t):
+  hoare [ToBytesSpec.remove_msb_if_set :
+      r = f3 /\ pow 2 63 <= W64.to_uint r < pow 2 64 ==> r = res - W64.of_int (pow 2 63)].
+proof. proc => />. wp; skip => />. move => *. rewrite helper_lemma_remove_msb. auto => />. ring. qed.
+
+lemma ph_remove_msb (r: W64.t):
+  phoare [ToBytesSpec.remove_msb_if_set : r = f3 /\ pow 2 63 <= W64.to_uint r < pow 2 64 ==>
+      r = res - W64.of_int (pow 2 63)] = 1%r.
+proof. by conseq ill_remove_msb_if_set (h_remove_msb r). qed.
 
 (** Extracts MSB **)
-lemma h_extract_msb_lt_2_255:
-  hoare [ToBytesSpec.extract_msb :
-      0 <= W64.to_uint f3 < pow 2 63
-      ==>
-      res = W64.zerow
-  ].
-    proc => />. wp; skip => /> &hr H H0.
-    rewrite /SAR_64 /shift_mask /rflags_OF //= sarE.
-    rewrite init_bits2w bits2wE -iotaredE /min //=.
-    rewrite upper_limb4_ltP_msbw //=.
-    + rewrite /W64.zerow /W64.zero bits2wE /int2bs /mkseq -iotaredE => />.
-qed.
+lemma h_extract_msb0:
+  hoare [ToBytesSpec.extract_msb : 0 <= W64.to_uint f3 < pow 2 63 ==> res = W64.zerow].
+proof. proc => />. wp; skip => /> &hr H H0. rewrite helper_lemma_extract_msb_0 /#. qed.
 
-lemma ph_extract_msb_lt_2_255:
-  phoare [ToBytesSpec.extract_msb :
-      0 <= W64.to_uint f3 < pow 2 63
-      ==>
-      res = W64.zerow] = 1%r.
-proof.
-    by conseq ill_extract_msb_lt_2_255 (h_extract_msb_lt_2_255).
-qed.
+lemma ph_extract_msb0:
+  phoare [ToBytesSpec.extract_msb : 0 <= W64.to_uint f3 < pow 2 63 ==> res = W64.zerow] = 1%r.
+proof. by conseq ill_extract_msb (h_extract_msb0). qed.
 
-(** Sets word to 19 if word = 0 **)
-lemma h_to19:
-  hoare [ToBytesSpec.to19 :
-      t = W64.zerow
-      ==>
-      res = W64.of_int 19
-  ].
-    proc => />. wp; skip => /> &hr H H0.
-qed.
+lemma h_extract_msb1:
+  hoare [ToBytesSpec.extract_msb : pow 2 63 <= W64.to_uint f3 < pow 2 64 ==> res = W64.onew].
+proof. proc => />. wp; skip => /> &hr H H0. rewrite helper_lemma_extract_msb_1. smt(). auto. qed.
 
+lemma ph_extract_msb1:
+  phoare [ToBytesSpec.extract_msb : pow 2 63 <= W64.to_uint f3 < pow 2 64 ==> res = W64.onew] = 1%r.
+proof. by conseq ill_extract_msb (h_extract_msb1). qed.
 
-lemma ph_to19:
-  phoare [ToBytesSpec.to19 :
-      t = W64.zerow
-      ==>
-      res = W64.of_int 19] = 1%r.
-proof.
-    by conseq ill_to19 (h_to19).
-qed.
+(** Sets word to 19 if word = 0 and 38 if word = 1 **)
+lemma h_to_19:
+  hoare [ToBytesSpec.to_19_or_38 : t = W64.zerow ==> res = W64.of_int 19].
+proof. proc => />. wp; skip => /> &hr H H0. qed.
 
-(** Adding 19 to a Rep4 **)
+lemma ph_to_19:
+  phoare [ToBytesSpec.to_19_or_38 : t = W64.zerow ==> res = W64.of_int 19] = 1%r.
+proof. by conseq ill_to_19_or_38 (h_to_19). qed.
 
-abbrev add19_l1 (r: Rep4) = (addc r.[0] ((of_int 19))%W64 false).`2.
-abbrev add19_l2 (r: Rep4) = (addc r.[1] W64.zero (addc_carry r.[0] ((of_int 19))%W64 false)).`2.
-abbrev add19_l3 (r: Rep4) = (addc r.[2] W64.zero (addc_carry r.[1] W64.zero (addc_carry r.[0] ((of_int 19))%W64 false))).`2.
-abbrev add19_l4 (r: Rep4) = (addc r.[3] W64.zero (addc_carry r.[2] W64.zero (addc_carry r.[1] W64.zero (addc_carry r.[0] ((of_int 19))%W64 false)))).`2.
+lemma h_to_38:
+  hoare [ToBytesSpec.to_19_or_38 : t = W64.onew ==> res = W64.of_int 38 ].
+proof. proc => />. wp; skip => /> &hr H H0. qed.
 
-abbrev add19 (r: Rep4) = Array4.of_list witness [add19_l1 r; add19_l2 r ; add19_l3 r ; add19_l4 r].
+lemma ph_to_38:
+  phoare [ToBytesSpec.to_19_or_38 : t = W64.onew ==> res = W64.of_int 38] = 1%r.
+proof. by conseq ill_to_19_or_38 (h_to_38). qed.
 
-lemma h_addition19 (r: Rep4):
+(** Adding 19 or 38 to a Rep4 **)
+lemma h_addition (r: Rep4, _tt1: W64.t, n : int):
   hoare [ToBytesSpec.addition :
-      r = f /\ operand2 = W64.of_int 19 /\  0 <= valRep4 r < p
+      r = f /\ _tt1 = _tt /\ operand2 = W64.of_int n /\ 19 <= n <= 38 /\ W64.to_uint _tt1 < pow 2 64-n
       ==>
-      res = add19 r /\ valRep4 r + 19 = valRep4 res
+      res = add_to_limb r _tt1 n /\
+      valRep4 (Array4.of_list witness [r.[0]; r.[1]; r.[2]; _tt1]) + n = valRep4 res
   ].
 proof.
-    proc. auto => />. move => &hr H H0. do split.
+    proc. auto => />. move => &hr H H0 H1. do split.
     + apply Array4.ext_eq => i ib. rewrite !addcE. rewrite !get_setE 1..4:/#.
     + case(i = 3) => C. rewrite C => />.
     + case(i = 2) => C0. rewrite C0 => />.
@@ -313,8 +707,8 @@ proof.
     + case(i = 0) => C2. rewrite C2 => />. smt().
     rewrite !addcE !/add_carry !/carry_add !b2i0 => />.
     rewrite !valRep4E !/to_list !/val_digits !/mkseq -!iotaredE => />.
-    rewrite !mulzDr -!mulzA !to_uintD !of_uintK (modz_small 19 (pow 2 64)) 1:/# => />.
-    case((18446744073709551616 <= u64i r.[0] + 19) = false) => C1. rewrite C1 !b2i0 => />.
+    rewrite !mulzDr -!mulzA !to_uintD !of_uintK (modz_small n (pow 2 64)) 1:/# => />.
+    case((18446744073709551616 <= u64i r.[0] + n) = false) => C1. rewrite C1 !b2i0 => />.
     + rewrite pmod_small. move: C1 W64.to_uint_cmp. smt().
     + rewrite pmod_small. move: W64.to_uint_cmp. smt().
     + rewrite pmod_small. move: W64.to_uint_cmp. smt().
@@ -328,14 +722,14 @@ proof.
     + rewrite (pmod_small (u64i r.[1] + 1 %% 18446744073709551616) 18446744073709551616).
     + move :W64.to_uint_cmp. smt(). auto => />.
     + rewrite (pmod_small (u64i r.[2]) 18446744073709551616). move: C1 W64.to_uint_cmp. smt().
-    + have ->: (u64i r.[0] + 19) %% 18446744073709551616 = (u64i r.[0] + 19) - 18446744073709551616.
+    + have ->: (u64i r.[0] + n) %% 18446744073709551616 = (u64i r.[0] + n) - 18446744073709551616.
     + move :W64.to_uint_cmp. smt(). move: W64.to_uint_cmp. smt().
 
     move: C2. rewrite not_false_to_true. move => C2. rewrite !C2 !b2i1.
     + rewrite (pmod_small 1 18446744073709551616). auto => />.
     + have ->: (u64i r.[1] + 1) %% 18446744073709551616 = (u64i r.[1] + 1) - 18446744073709551616.
     + move: W64.to_uint_cmp. smt().
-    + have ->: (u64i r.[0] + 19) %% 18446744073709551616 = (u64i r.[0] + 19) - 18446744073709551616.
+    + have ->: (u64i r.[0] + n) %% 18446744073709551616 = (u64i r.[0] + n) - 18446744073709551616.
     + move: W64.to_uint_cmp. smt().
 
     case(18446744073709551616 <= u64i r.[2] + 1 = false) => C3. rewrite C3 b2i0 => />.
@@ -343,449 +737,587 @@ proof.
     + rewrite pmod_small. move: W64.to_uint_cmp. smt(). ring.
 
     move: C3. rewrite not_false_to_true. move => C3. rewrite !C3 !b2i1 => />.
+
     + have ->: (u64i r.[2] + 1) %% 18446744073709551616 = (u64i r.[2] + 1) - 18446744073709551616.
     + move: W64.to_uint_cmp. smt().
-    + have E: 0 <= u64i r.[3] && u64i r.[3] < pow 2 63.
-    + apply upper_limb4_ltP_range. smt().
+    + have E: 0 <= u64i _tt1 && u64i _tt1 < pow 2 64.
+    + move: W64.to_uint_cmp. smt().
     + rewrite pmod_small. move: E. smt().
     ring.
 qed.
 
-lemma ph_addition19 (r: Rep4):
+lemma ph_addition (r: Rep4, _tt1: W64.t, n : int):
   phoare [ToBytesSpec.addition :
-      r = f /\ operand2 = W64.of_int 19 /\  0 <= valRep4 r < p
+      r = f /\ _tt1 = _tt /\ operand2 = W64.of_int n /\ 19 <= n <= 38  /\ W64.to_uint _tt1 < pow 2 64 - n
       ==>
-      res = add19 r /\ valRep4 r + 19 = valRep4 res
+      res = add_to_limb r _tt1 n /\
+      valRep4 (Array4.of_list witness [r.[0]; r.[1]; r.[2]; _tt1]) + n = valRep4 res
   ] = 1%r.
-proof.
-    by conseq ill_addition (h_addition19 r).
-qed.
+proof. by conseq ill_addition (h_addition r _tt1 n). qed.
 
-lemma h_addition19_calls (r: Rep4):
-  equiv [ToBytesSpec.addition_calls ~ ToBytesSpec.addition :
-      0 <= valRep4 f{1} < p /\ ={f} /\ operand2{2} = W64.of_int 19
-      ==>
-       valRep4 res{1} = valRep4 res{2}
-  ].
-proof.
-    proc *. auto => />. inline {1} 1.
-    seq 3 0 : (#pre /\ f0{1} = f{2} /\ ff{1} = witness /\ extracted_msbw{1} = W64.zerow).
-    + ecall {1} (ph_extract_msb_lt_2_255). auto => />.
-    + move => &2 H H0.
-    + move: upper_limb4_ltP_range r. smt().
-    seq 1 0 : (#pre /\ tt{1} = f0{1}.[3]).
-    + ecall {1} (ph_remove_msb_if_set_lt_2_255 (f0{1}.[3])).
-    + auto => />. move => &1 &2 [#] H. do split.
-    + move: (upper_limb4_ltP_range (f{1})) (W64.to_uint_cmp f{1}.[3]). auto => />.
-    + move: (upper_limb4_ltP_range (f{1})) (W64.to_uint_cmp f{1}.[3]). auto => />. smt().
-    seq 1 0 : (#pre /\ tt0{1} = W64.of_int 19).
-    + ecall {1} (ph_to19). auto => />. wp.
-    ecall {1} (ph_addition19 (f0{1})).
-    ecall {2} (ph_addition19 (f{2})).
-    auto => />.
-qed.
-
-(** Substraction **)
-lemma h_subtraction19 (r: Rep4):
+(** Substraction of 0, 19 or 38 to a Rep4 **)
+lemma h_subtraction (r: Rep4, n: int):
   hoare [ToBytesSpec.subtraction :
-      r = f /\ operand2 = W64.of_int 19 /\ 19 <= valRep4 r < W256.modulus
+      r = f /\ operand2 = W64.of_int n /\ 19 <= n <= 38 /\ n <= valRep4 r < W256.modulus
       ==>
-      valRep4 r - 19 = valRep4 res
+      res = sub_from_limb r n /\ valRep4 r - n = valRep4 res
   ].
 proof.
-    proc. auto => />. move => &hr H H0.
+    proc. auto => />. move => &hr H H0 H1 H2.
+    do split.
+    + apply Array4.ext_eq => i ib. rewrite !subcE. rewrite !get_setE 1..4:/#.
+    + case(i = 3) => C. rewrite C => />.
+    + case(i = 2) => C0. rewrite C0 => />.
+    + case(i = 1) => C1. rewrite C1 => />.
+    + case(i = 0) => C2. rewrite C2 => />. smt().
+
     rewrite !subcE !/borrow_sub !b2i0 => />.
     rewrite !valRep4E !/to_list !/val_digits !/mkseq -!iotaredE => />.
-    rewrite !mulzDr -!mulzA !to_uintD !to_uintN (modz_small 19 (pow 2 64)) 1:/# => />.
+    rewrite !mulzDr -!mulzA !to_uintD !to_uintN !of_uintK (modz_small n (pow 2 64)) 1:/# => />.
 
-    case ((u64i r.[0] < 19) = false) => C1. rewrite !C1 !b2i0 !to_uint0 => />.
+    case ((u64i r.[0] < n) = false) => C1. rewrite !C1 !b2i0 => />.
     have ->: u64i r.[1] < 0 = false. move: W64.to_uint_cmp; 1:smt().
     have ->: u64i r.[2] < 0 = false. move: W64.to_uint_cmp; 1:smt().
     rewrite !b2i0 => />.
-    + have ->: (u64i r.[0] + 18446744073709551597) %% 18446744073709551616 =
-               (u64i r.[0] + 18446744073709551597) - 18446744073709551616.
-    + move: W64.to_uint_cmp. smt(). auto => />.
+    + have ->: (u64i r.[0] + (-n) %% 18446744073709551616) %% 18446744073709551616 =
+               (u64i r.[0] + (-n) %% 18446744073709551616) - 18446744073709551616.
+    + move: W64.to_uint_cmp. smt(). auto => />. rewrite !modNz 1,2:/#.
+    + rewrite pmod_small. move: W64.to_uint_cmp. smt().
     + rewrite pmod_small. move: W64.to_uint_cmp. smt().
     + rewrite pmod_small. move: W64.to_uint_cmp. smt().
     + rewrite pmod_small. move: W64.to_uint_cmp. smt().
     + ring.
 
-    move: C1. rewrite not_false_to_true. move => C1. rewrite !C1 !b2i1 !to_uint1 => />.
+    move: C1. rewrite not_false_to_true. move => C1. rewrite !C1 !b2i1 => />.
     rewrite pmod_small. move: W64.to_uint_cmp. smt().
-    case ((u64i r.[1] < 1) = false) => C2. rewrite !C2 !b2i0 !to_uint0 => />.
+    case ((u64i r.[1] < 1) = false) => C2. rewrite !C2 !b2i0  => />.
     + have ->: u64i r.[2] < 0 = false. move: W64.to_uint_cmp; 1:smt().
     + rewrite !b2i0 => />.
     + have ->: (u64i r.[1] + 18446744073709551615) %% 18446744073709551616 =
                (u64i r.[1] + 18446744073709551615) - 18446744073709551616.
     + move: W64.to_uint_cmp. smt(). auto => />.
+    + rewrite !modNz 1,2:/#.
+    + rewrite pmod_small. move: W64.to_uint_cmp. smt().
     + rewrite pmod_small. move: W64.to_uint_cmp. smt().
     + rewrite pmod_small. move: W64.to_uint_cmp. smt().
     + ring.
 
-    move: C2. rewrite not_false_to_true. move => C2. rewrite !C2 !b2i1 !to_uint1 => />.
+    move: C2. rewrite not_false_to_true. move => C2. rewrite !C2 !b2i1 => />.
+    + rewrite modNz 1,2:/#.
     rewrite pmod_small. move: W64.to_uint_cmp. smt().
-    case ((u64i r.[2] < 1) = false) => C3. rewrite !C3 !b2i0 !to_uint0 => />.
+    case ((u64i r.[2] < 1) = false) => C3. rewrite !C3 !b2i0  => />.
     + have ->: (u64i r.[2] + 18446744073709551615) %% 18446744073709551616 =
                (u64i r.[2] + 18446744073709551615) - 18446744073709551616.
     + move: W64.to_uint_cmp. smt(). auto => />.
     + rewrite pmod_small. move: W64.to_uint_cmp. smt().
+    + rewrite pmod_small. move: W64.to_uint_cmp. smt().
     + ring.
 
-    move: C3. rewrite not_false_to_true. move => C3. rewrite !C3 !b2i1 !to_uint1 => />.
+    move: C3. rewrite not_false_to_true. move => C3. rewrite !C3 !b2i1 => />.
     rewrite pmod_small. move: W64.to_uint_cmp. smt().
     have E: ((u64i r.[3] < 1) = false).
-    + move: (W64.to_uint_cmp r.[3])  (upper_limb4_ltP_range r) H H0.
+    + move: (W64.to_uint_cmp r.[3])  (limb4_ltP_cmp r) H H0 H2 H1.
     + rewrite !valRep4E !pE !/to_list !/val_digits !/mkseq -!iotaredE => />.
-    + rewrite !mulzDr -!mulzA   (modz_small 0 (pow 2 64)) 1:/# => />; 1:smt().
+    + rewrite !mulzDr -!mulzA   (pmod_small 0 (pow 2 64)) 1:/# => />. smt().
     + have ->: (u64i r.[3] + 18446744073709551615) %% 18446744073709551616 =
                (u64i r.[3] + 18446744073709551615) - 18446744073709551616.
-    + move: W64.to_uint_cmp. smt(). auto => />. ring.
+    + move: W64.to_uint_cmp. smt(). auto => />.
+    + rewrite pmod_small. move: W64.to_uint_cmp. smt(). ring.
 qed.
 
-lemma ph_subtraction19 (r: Rep4):
-  phoare [ToBytesSpec.subtraction :
-       r = f /\ operand2 = W64.of_int 19 /\ 19 <= valRep4 r < W256.modulus
+lemma h_subtraction0 (r: Rep4, n: int):
+  hoare [ToBytesSpec.subtraction :
+      r = f /\ operand2 = W64.of_int n /\ n = 0 /\ n <= valRep4 r < W256.modulus
       ==>
-      valRep4 r - 19 = valRep4 res
-  ] = 1%r.
+      res = sub_from_limb r n /\ valRep4 r - n = valRep4 res
+  ].
 proof.
-    by conseq ill_subtraction (h_subtraction19 r).
+    proc. auto => />. move => &hr H H0.
+    do split.
+    + apply Array4.ext_eq => i ib. rewrite !subcE. rewrite !get_setE 1..4:/#.
+    + case(i = 3) => C. rewrite C => />.
+    + case(i = 2) => C0. rewrite C0 => />.
+    + case(i = 1) => C1. rewrite C1 => />.
+    + case(i = 0) => C2. rewrite C2 => />. smt().
+
+    rewrite !subcE !/borrow_sub !b2i0 => />.
+    rewrite !valRep4E !/to_list !/val_digits !/mkseq -!iotaredE => />.
+    rewrite !mulzDr -!mulzA !to_uintD !to_uintN !of_uintK.
+    have ->: u64i r.[0] < 0 = false. move: W64.to_uint_cmp; 1:smt().
+    have ->: u64i r.[1] < 0 = false. move: W64.to_uint_cmp; 1:smt().
+    have ->: u64i r.[2] < 0 = false. move: W64.to_uint_cmp; 1:smt().
+    rewrite !b2i0. auto => />.
+    rewrite pmod_small. move: W64.to_uint_cmp. smt().
+    rewrite pmod_small. move: W64.to_uint_cmp. smt().
+    rewrite pmod_small. move: W64.to_uint_cmp. smt().
+    rewrite pmod_small. move: W64.to_uint_cmp. smt().
+    ring.
+qed.
+
+
+lemma ph_subtraction (r: Rep4, n: int):
+  phoare [ToBytesSpec.subtraction :
+      r = f /\ operand2 = W64.of_int n /\ 19 <= n <= 38 /\ n <= valRep4 r < W256.modulus
+      ==>
+      res = sub_from_limb r n /\ valRep4 r - n = valRep4 res
+  ] = 1%r.
+proof. by conseq ill_subtraction (h_subtraction r n). qed.
+
+lemma ph_subtraction0 (r: Rep4, n: int):
+  phoare [ToBytesSpec.subtraction :
+      r = f /\ operand2 = W64.of_int n /\ n = 0 /\ n <= valRep4 r < W256.modulus
+      ==>
+      res = sub_from_limb r n /\ valRep4 r - n = valRep4 res
+  ] = 1%r.
+proof. by conseq ill_subtraction (h_subtraction0 r n). qed.
+
+
+(** To Bytes **)
+lemma h_to_bytes_no_reduction (r: Rep4):
+  hoare [ToBytesSpec.to_bytes :
+      r = f /\ 0 <= valRep4 r < p
+      ==>
+      valRep4 res = asint (inzpRep4 r)
+  ].
+proof.
+    proc.
+    seq 9: (#pre /\ valRep4 ff3 = valRep4 r).
+    seq 1 : (#pre /\ msb1 = W64.zerow). call h_extract_msb0. auto => />.
+    + move: (limb4_ltP_cmp r). smt(limb4_ltP_cmp).
+    seq 1 : (#pre /\ _tt = f.[3]). call (h_msb_not_set (r.[3])). auto => />.
+    + move: (limb4_ltP_cmp r). smt().
+    seq 1 : (#pre /\ _tt0 = W64.of_int 19). call h_to_19. auto => />.
+    seq 1 : (#pre /\ valRep4 r + 19 = valRep4 ff
+                  /\ (add_to_limb r _tt 19) = ff). call (h_addition r r.[3] 19). auto => />.
+    + apply limb4_add_equiv_ltP.
+    seq 1 : (#pre /\ _f3 = ff.[3]). call (h_msb_not_set (add_to_limb r r.[3] 19).[3]). auto => />.
+    + apply limb4_add19_range_l4_ltP. sp.
+    seq 1 : (#pre /\ _tt2 = W64.of_int 19). auto => />. call h_to_19_by_invw.
+    + auto => />. apply limb4_add19_range_l4_ltP.
+    call (h_subtraction (add_to_limb r r.[3] 19) 19). auto => />.
+    move => &hr [#] H H0. do split.
+    + apply Array4.ext_eq => i ib. rewrite !get_setE 1:/#.
+    + case(i = 3) => C. rewrite C => />.
+    + case(i = 2) => C0. rewrite C0 => />.
+    + case(i = 1) => C1. rewrite C1 => />.
+    + case(i = 0) => C2. rewrite C2 => />. smt().
+    + rewrite -H0. move: valRep4_cmp. smt(). move => H2.
+    + rewrite -H0. move: valRep4_cmp. smt(). move => H3 H4 H5 H6. smt().
+    auto => />. smt(cminusP0).
 qed.
 
 (** To Bytes **)
-lemma h_tobytes_no_reduction (r: Rep4):
-  hoare [ToBytesSpec.tobytes_no_reduction :
-      r = f /\ 0 <= valRep4 r < p
+lemma h_to_bytes_cminusP_part1 (r: Rep4):
+  hoare [ToBytesSpec.to_bytes :
+      r = f /\ p <= valRep4 r < pow 2 255
       ==>
-      valRep4 r = valRep4 res
+      valRep4 res = asint (inzpRep4 r)
+      (* valRep4 r - p = valRep4 res *)
   ].
 proof.
-    proc. inline 1.
-    seq 3 : (#pre /\ extracted_msbw0 = W64.zerow /\ f0 = f).
-    + call h_extract_msb_lt_2_255. auto => />.
-    + move => H H0. move: (upper_limb4_ltP_range r). smt().
-    seq 1 : (#pre /\ tt1 = f.[3]).
-    + call (h_remove_msb_if_set_lt_2_255 (r.[3])). auto => />.
-    + move: (upper_limb4_ltP_range r). smt().
-    seq 1 : (#pre /\ tt00 = W64.of_int 19).
-    + call h_to19. auto => />.
-    + seq 1 : (#pre /\ valRep4 r + 19 = valRep4 ff0 /\ add19 r = ff0).
-    + call (h_addition19 r). auto => />.
-    seq 2 : (#pre /\ f3 = W64.of_int 19 /\ ff = ff0).
-    + call h_sar_inv_t. auto => />.
-    + move => &hr.
-    rewrite !addcE !/add_carry !/carry_add !b2i0 => />.
-    rewrite !valRep4E !pVal !/to_list !/val_digits !/mkseq -!iotaredE => />.
-    rewrite !mulzDr -!mulzA !to_uintD !of_uintK (modz_small 19 (pow 2 64)) 1:/# => />.
-    + move: (upper_limb4_ltP_range r).
-    + move: (W64.to_uint_cmp (add19_l4 r)). smt().
-    call (h_subtraction19 (add19 r)). auto => />.
-    move => &hr [#] H H0. do split;1:smt(). move: H.
-    rewrite pVal 1:/#. smt().
+    proc.
+    seq 9: (#pre /\ valRep4 ff3 = valRep4 r - p).
+    seq 1 : (#pre /\ msb1 = W64.zerow). call h_extract_msb0. auto => />.
+    + move: (limb4_lt_2_255_cmp r) pVal. smt().
+    seq 1 : (#pre /\ _tt = f.[3]). call (h_msb_not_set (r.[3])). auto => />.
+    + move: (limb4_lt_2_255_cmp r) pVal. smt().
+    seq 1 : (#pre /\ _tt0 = W64.of_int 19). call h_to_19. auto => />.
+    seq 1 : (#pre /\ valRep4 r + 19 = valRep4 ff
+                  /\ (add_to_limb r _tt 19) = ff). call (h_addition r r.[3] 19). auto => />.
+    + apply limb4_add_equiv_geqP_lt_2p. swap 2 1.
+    seq 1 : (#pre /\ _f3 = ff.[3] - W64.of_int (pow 2 63)). inline 1. auto => />.
+    + move => H H0 H1. rewrite helper_lemma_remove_msb.
+    + move: limb4_add_range_geqP_lt_2_255. smt(). auto.
+    seq 1 : (#pre /\ _tt2 = W64.of_int 0). call h_to_0_by_invw. auto => />.
+    + apply limb4_add_range_geqP_lt_2_255.
+    seq 1 : (#pre /\ valRep4 ff2 = valRep4 ff - (pow 2 255) /\ ff2 = ff.[3 <- _f3]).
+    auto => />. apply limb4_set_f3_geq_2_255_lt_2p.
+    call (h_subtraction0 (add_to_limb r r.[3] 19).[3 <-
+            (add_to_limb r r.[3] 19).[3] - (of_int (pow 2 63))%W64] 0). auto => />.
+    move => [#] H H0 H1 H2. do split.
+    + move: valRep4_cmp. smt(). move => H3.
+    + move: valRep4_cmp. smt(). move => H4 H5 H6.
+    + rewrite -H6. move : H H0 H1 H2 H4 H5 H6.
+    + rewrite !valRep4E !pVal !/to_list !/val_digits !/mkseq -!iotaredE => />.
+    + move: W64.to_uint_cmp. rewrite !addcE !/carry_add !b2i0 => />. smt().
+    auto => />. smt(pVal cminusP1).
 qed.
 
+
+lemma h_to_bytes_cminusP_part2 (r: Rep4):
+  hoare [ToBytesSpec.to_bytes :
+      r = f /\ pow 2 255 <= valRep4 r < 2*p
+      ==>
+      valRep4 res = asint (inzpRep4 r)
+      (* valRep4 r - p = valRep4 res *)
+  ].
+proof.
+    proc.
+    seq 9: (#pre /\ valRep4 ff3 = valRep4 r - p).
+    seq 1 : (#pre /\ msb1 = W64.onew). call h_extract_msb1. auto => />.
+    + move => H H0. move: (limb4_geq_2_255_cmp r) pVal. smt().
+    seq 1 : (#pre /\ _tt = f.[3] - W64.of_int (pow 2 63)
+                  /\ W64.to_uint _tt = W64.to_uint f.[3] - (pow 2 63)).
+    + inline 1. auto => />. move => H H0. rewrite helper_lemma_remove_msb.
+    + move: limb4_geq_2_255_cmp W64.to_uint_cmp H H0 pVal. smt(). do split.
+    + move: H H0. apply limb4_minus_2_63_equiv.
+    seq 1 : (#pre /\ _tt0 = W64.of_int 38). call h_to_38. auto => />.
+    seq 1 : (#pre /\ valRep4 r - pow 2 255 + 38 = valRep4 ff /\ (add_to_limb r _tt 38) = ff).
+    + call (h_addition r (r.[3] - W64.of_int (pow 2 63)) 38). auto => />.
+    + apply limb4_add_sub_equiv_geqP_lt_2p. swap 3 -1.
+    seq 1 : (#pre /\ _f3 = ff.[3]). inline 1. auto => />.
+    + apply limb4_minus_2_63_add38_equiv.
+    seq 1 : (#pre /\ _tt2 = W64.of_int 19). call h_to_19_by_invw. auto => />.
+    + apply limb4_add_range_geq_2_255_lt_2p.
+    seq 1 : (#pre /\ valRep4 ff2 = valRep4 ff /\ ff2 = ff.[3 <- _f3]). auto => />.
+    + apply limb4_set_f3_gtP_lt_2p.
+    call (h_subtraction ((add_to_limb r (r.[3] - (of_int 9223372036854775808)%W64) 38).[3 <-
+            add_l4 r (r.[3] - (of_int 9223372036854775808)%W64) 38]) 19). auto => />.
+    move => [#] H H0 H1 H2 H3. do split.
+    + move: valRep4_cmp. smt(). move => H4.
+    + move: valRep4_cmp. smt(). move => H4 H5 H6.
+    + rewrite -H6. move : H H0 H1 H2 H4 H5 H6.
+    + rewrite !valRep4E !pVal !/to_list !/val_digits !/mkseq -!iotaredE => />.
+    + move: W64.to_uint_cmp. rewrite !addcE !/carry_add !b2i0 => />. smt().
+    + auto => />. smt(pVal cminusP1).
+qed.
+
+lemma h_to_bytes_cminus2P (r: Rep4):
+  hoare [ToBytesSpec.to_bytes :
+      r = f /\ 2*p <= valRep4 r < W256.modulus
+      ==>
+      valRep4 res = asint (inzpRep4 r)
+      (* valRep4 r - p - p = valRep4 res *)
+  ].
+proof.
+    proc.
+    seq 9: (#pre /\ valRep4 ff3 = valRep4 r - p - p).
+    seq 1 : (#pre /\ msb1 = W64.onew). call h_extract_msb1. auto => />.
+    + move => H H0. move: (limb4_geq_2_255_cmp r) pVal. smt().
+    seq 1 : (#pre /\ _tt = f.[3] - W64.of_int (pow 2 63)
+                  /\ W64.to_uint _tt = W64.to_uint f.[3] - (pow 2 63)).
+    + inline 1. auto => />. move => H H0. rewrite helper_lemma_remove_msb.
+    + move: limb4_geq_2_255_cmp W64.to_uint_cmp H H0 pVal. smt(). do split.
+    + move: H H0. apply limb4_minus_2_63_equiv_2.
+    seq 1 : (#pre /\ _tt0 = W64.of_int 38). call h_to_38. auto => />.
+    seq 1 : (#pre /\ valRep4 r - pow 2 255 + 38 = valRep4 ff /\ (add_to_limb r _tt 38) = ff).
+    + call (h_addition r (r.[3] - W64.of_int (pow 2 63)) 38). auto => />.
+    + apply limb4_add_sub_equiv_geq2P.
+    seq 1 : (#pre /\ _f3 = ff.[3] - W64.of_int (pow 2 63)). inline 1. auto => />.
+    + apply limb4_minus_2_63_add38_equiv_2. swap 1 1.
+    seq 1 : (#pre /\ _tt2 = W64.of_int 0). call h_to_0_by_invw. auto => />.
+    + apply limb4_add_range_geq2P.
+    seq 1 : (#pre /\ valRep4 ff2 = valRep4 ff - (pow 2 255) /\ ff2 = ff.[3 <- _f3]). auto => />.
+    + apply limb4_set_f3_gt2P.
+    call (h_subtraction0 ((add_to_limb r (r.[3] - (of_int 9223372036854775808)%W64) 38).[3 <-
+        add_l4 r (r.[3] - (of_int 9223372036854775808)%W64) 38
+            - (of_int 9223372036854775808)%W64]) 0). auto => />.
+    move => &hr [#] H H0 H1 H2. do split.
+    + move: valRep4_cmp. smt(). move => H3.
+    + move: valRep4_cmp. smt(). move => H4 H5 H6.
+    + rewrite -H6 H2 -H1 !pVal. smt().
+    auto => />. move => &hr. move => H H1 H2. rewrite H2 cminusP2. move: H valRep4_cmp. smt().
+    by rewrite inzpRep4E.
+qed.
+
+
+lemma equiv_to_bytes:
+    equiv[M.__tobytes4 ~ ToBytesSpec.to_bytes :
+      f{1} = f{2}
+      ==>
+      valRep4 res{1} = valRep4 res{2}
+    ].
+proof.
+    proc => />.
+    swap {2} 2 -1. swap{1} 9 -7. swap {1} 24 -1. inline *.
+    inline *.
+    inline {2} 1.
+    seq 2 4 : (#pre /\ _tt{2} = t{1} /\ _tt{2} = (f.[3]{2} + f.[3]{2}) `>>` W8.one). auto => />.
+    inline {2} 1.
+    seq  7 9 : (_tt{2} = t{1} /\ msb1{2} = f.[3]{1} /\
+                f.[0]{1} = f.[0]{2} /\
+                f.[1]{1} = f.[1]{2} /\
+                f.[2]{1} = f.[2]{2} /\
+                _tt{2} = (f.[3]{2} + f.[3]{2}) `>>` W8.one /\
+                msb1{2} = (SAR_64 f{2}.[3] ((of_int 63))%W8).`6). auto => />.
+    inline {2} 1.
+    seq  2 4 : (_tt{2} = t{1} /\
+                _tt{2} = (f.[3]{2} + f.[3]{2}) `>>` W8.one /\
+                f.[0]{1} = f.[0]{2} /\
+                f.[1]{1} = f.[1]{2} /\
+                f.[2]{1} = f.[2]{2} /\
+                msb1{2} = (SAR_64 f{2}.[3] ((of_int 63))%W8).`6 /\
+                _tt0{2} = f.[3]{1} /\ _tt0{2} = msb1{2} `&` W64.of_int 19 + W64.of_int 19 ). auto => />.
+    inline {2} 1.
+    seq  10 15 : (_tt{2} = (f.[3]{2} + f.[3]{2}) `>>` W8.one /\
+                 msb1{2} = (SAR_64 f{2}.[3] ((of_int 63))%W8).`6 /\
+                 _tt0{2} = msb1{2} `&` W64.of_int 19 + W64.of_int 19 /\
+                 f0{2} = f{2} /\ _tt0{2} = f.[3]{1} /\
+                 tt0{2} = t{1} /\
+                 (* ff0{2} = add_to_limb f0{2} _tt{2} (W64.to_uint tt0{2}) /\ *)
+                 ff0{2}.[0] = add_l1 f0{2} (W64.to_uint _tt0{2}) /\
+                 ff0{2}.[1] = add_l2 f0{2} (W64.to_uint _tt0{2}) /\
+                 ff0{2}.[2] = add_l3 f0{2} (W64.to_uint _tt0{2}) /\
+                 ff0{2}.[3] = add_l4 f0{2} _tt{2} (W64.to_uint _tt0{2}) /\
+                 f.[0]{1} = ff0.[0]{2} /\ f.[1]{1} = ff0.[1]{2} /\
+                 f.[2]{1} = ff0.[2]{2} /\ ff{2} = ff0{2} /\ ff{2}.[3] = t{1}). auto => />.
+    move => &1 &2 [#] H H0 H1 H2. do split.
+    rewrite H H0 H1 H2 //=. rewrite H //=. rewrite H H0 //=. rewrite H H0 H1 //=.
+    rewrite H H0 H1 //=.
+    swap {2} 2 -1. swap {2} 4 -2. swap {1} 2 1.
+    inline {2} 1.
+    seq  2 5 : (_tt{2} = (f.[3]{2} + f.[3]{2}) `>>` W8.one /\
+                 msb1{2} = (SAR_64 f{2}.[3] ((of_int 63))%W8).`6 /\
+                 _tt0{2} = msb1{2} `&` W64.of_int 19 + W64.of_int 19 /\
+                 f0{2} = f{2} /\
+                 f.[3]{1} = _f3{2} /\
+                 _f3{2} = (ff.[3]{2} + ff.[3]{2}) `>>` W8.one /\
+                 (* ff0{2} = add_to_limb f0{2} _tt{2} (W64.to_uint tt0{2}) /\ *)
+                 ff0{2}.[0] = add_l1 f0{2} (W64.to_uint _tt0{2}) /\
+                 ff0{2}.[1] = add_l2 f0{2} (W64.to_uint _tt0{2}) /\
+                 ff0{2}.[2] = add_l3 f0{2} (W64.to_uint _tt0{2}) /\
+                 ff0{2}.[3] = add_l4 f0{2} _tt{2} (W64.to_uint _tt0{2}) /\
+                 ff2{2} = ff{2}.[3 <- _f3{2}] /\
+                 ff2{2}.[3] = f{1}.[3] /\
+                 f.[0]{1} = ff0.[0]{2} /\ f.[1]{1} = ff0.[1]{2} /\
+                 f.[2]{1} = ff0.[2]{2} /\ ff{2} = ff0{2} /\ ff{2}.[3] = t{1}). auto => />.
+    inline {2} 1.
+    seq 1 9 : (_tt{2} = (f.[3]{2} + f.[3]{2}) `>>` W8.one /\
+                 msb1{2} = (SAR_64 f{2}.[3] ((of_int 63))%W8).`6 /\
+                 _tt0{2} = msb1{2} `&` W64.of_int 19 + W64.of_int 19 /\
+                 f0{2} = f{2} /\
+                 f.[3]{1} = _f3{2} /\
+                 _f3{2} = (ff.[3]{2} + ff.[3]{2}) `>>` W8.one /\
+                 (* ff0{2} = add_to_limb f0{2} _tt{2} (W64.to_uint tt0{2}) /\ *)
+                 ff0{2}.[0] = add_l1 f0{2} (W64.to_uint _tt0{2}) /\
+                 ff0{2}.[1] = add_l2 f0{2} (W64.to_uint _tt0{2}) /\
+                 ff0{2}.[2] = add_l3 f0{2} (W64.to_uint _tt0{2}) /\
+                 ff0{2}.[3] = add_l4 f0{2} _tt{2} (W64.to_uint _tt0{2}) /\
+                 ff2{2} = ff{2}.[3 <- _f3{2}] /\
+                 ff2{2}.[3] = f{1}.[3] /\
+                 f.[0]{1} = ff0.[0]{2} /\ f.[1]{1} = ff0.[1]{2} /\
+                 f.[2]{1} = ff0.[2]{2} /\ ff{2} = ff0{2} /\
+                 msb2{2} = (SAR_64 ff{2}.[3] ((of_int 63))%W8).`6 /\
+                 msb2{2} = t{1}). auto => />.
+    inline {2} 1.
+    inline {2} 1.
+    seq 1 9 : (_tt{2} = (f.[3]{2} + f.[3]{2}) `>>` W8.one /\
+                 msb1{2} = (SAR_64 f{2}.[3] ((of_int 63))%W8).`6 /\
+                 _tt0{2} = msb1{2} `&` W64.of_int 19 + W64.of_int 19 /\
+                 f0{2} = f{2} /\
+                 f.[3]{1} = _f3{2} /\
+                 _f3{2} = (ff.[3]{2} + ff.[3]{2}) `>>` W8.one /\
+                 (* ff0{2} = add_to_limb f0{2} _tt{2} (W64.to_uint tt0{2}) /\ *)
+                 ff0{2}.[0] = add_l1 f0{2} (W64.to_uint _tt0{2}) /\
+                 ff0{2}.[1] = add_l2 f0{2} (W64.to_uint _tt0{2}) /\
+                 ff0{2}.[2] = add_l3 f0{2} (W64.to_uint _tt0{2}) /\
+                 ff0{2}.[3] = add_l4 f0{2} _tt{2} (W64.to_uint _tt0{2}) /\
+                 ff2{2} = ff{2}.[3 <- _f3{2}] /\
+                 ff2{2}.[3] = f{1}.[3] /\
+                 f.[0]{1} = ff0.[0]{2} /\ f.[1]{1} = ff0.[1]{2} /\
+                 f.[2]{1} = ff0.[2]{2} /\ ff{2} = ff0{2} /\
+                 msb2{2} = (SAR_64 ff{2}.[3] ((of_int 63))%W8).`6 /\
+                 msb2{2} = t{1}). auto => />.
+    + apply Array4.ext_eq => i ib. rewrite !addcE !/carry_add !b2i0 => />.
+    rewrite !get_setE 1..4:/#.
+    + case(i = 3) => C. rewrite C => />.
+    + case(i = 2) => C0. rewrite C0 => />.
+    + case(i = 1) => C1. rewrite C1 => />.
+    + case(i = 0) => C2. rewrite C2 => />. smt().
+
+    seq 2 1: (#pre /\ t{1} = _tt{2} /\ _tt{2} = f{2}.[3] /\ 0 <= valRep4 f{2} < p).
+    + ecall {2} (ph_msb_not_set f{2}.[3]). auto => />.
+    + move => &2. do split.
+    + smt(W64.to_uint_cmp).
+    + move: limb4_lt_2_255_cmp W64.to_uint_cmp pVal; 1:smt().
+    + move => H1 H2. rewrite helper_lemma_msb_is_not_set /#.
+
+    seq 6 1 : (#pre /\ extracted_msbw{2} = W64.zerow /\ aux_4{1} = extracted_msbw{2}).
+    + auto => />. ecall {2} (ph_extract_msb0). auto => />.
+    + move => &2 H H0. do split.
+    + smt(W64.to_uint_cmp).
+    + move: H H0 limb4_ltP_cmp. smt(). move => *.
+    + rewrite helper_lemma_extract_msb_0 /#.
+
+    seq 1 0 : (0 <= valRep4 f{1} && valRep4 f{1} < p - W64.to_uint (f.[3]{2}) /\ t{1} = _tt{2}
+               /\ _tt{2} = f{2}.[3] /\
+               0 <= valRep4 f{2} && valRep4 f{2} < p /\ extracted_msbw{2} = W64.zerow /\
+               aux_4{1} = extracted_msbw{2} /\
+               f{1} = Array4.of_list witness [f.[0]{2}; f.[1]{2}; f.[2]{2}; extracted_msbw{2}]).
+    + auto => />. move => &2 H H0. do split.
+    + rewrite valRep4_cmp //=. move => H3. do split.
+    + rewrite valRep4_remove_limb4_ltP //=.
+    + rewrite valRep4_remove_limb4_ltP_structure //=.
+
+    seq 2 1 : (0 <= valRep4 f{1} && valRep4 f{1} < p - (W64.to_uint f.[3]{2}) + 19 * pow 2 192 /\
+               t{1} = _tt{2} /\ _tt{2} = f{2}.[3] /\ 0 <= valRep4 f{2} && valRep4 f{2} < p
+               /\ extracted_msbw{2} = W64.zerow /\
+               tt0{2} = W64.of_int 19 /\  /\
+               f{1} = Array4.of_list witness [f.[0]{2}; f.[1]{2}; f.[2]{2}; tt0{2}]).
+   + ecall {2} (ph_to_19). auto => />. move => &2 [#] H H0 H1 H2.
+   + have E: W64.zerow `&` (of_int 19)%W64 + (of_int 19)%W64 = W64.of_int 19. smt(@W64).
+   + do split. rewrite valRep4_cmp //=. move => H3. do split.
+   + move: H H0. rewrite !valRep4E pE !/to_list !/val_digits !/mkseq -!iotaredE => />.
+   + rewrite E to_uint0 //=. smt(W64.to_uint_cmp).
+   + rewrite E. apply Array4.ext_eq => i ib. rewrite get_setE //=. smt(Array4.initE).
+
+    seq 10 1 : (0 <= valRep4 f{2} && valRep4 f{2} < p
+               /\ extracted_msbw{2} = W64.zerow /\ _tt{2} = f{2}.[3]
+               /\ tt0{2} = W64.of_int 19 /\ 19 <= valRep4 ff{2} && valRep4 ff{2} < p+19 /\
+               ff{2} = (add_to_limb f{2} _tt{2} 19) /\ f{1}.[0] = add_l1 f{2} 19 /\
+               f{1}.[1] = add_l2 f{2} 19 /\ _tt{2} = f{2}.[3] /\
+               f{1}.[2] = add_l3 f{2} 19 /\ f{1}.[3] = W64.of_int 19  /\ t{1} = add_l4 f{2} _tt{2} 19).
+   + ecall {2} (ph_addition f{2} _tt{2} 19). auto => />. move => &1 [#] H H0 H1 H2.
+   + do split. move: H2. rewrite pVal 1:/#. move: limb4_ltP_cmp. move: H1 H2. smt().
+   move => H3 H4 H5. do split. rewrite -H5. move: valRep4_cmp. smt(). move => H6.
+   rewrite -H5 pVal. rewrite -valRep4_equiv_representation. move: H2. rewrite pVal 1:/#.
+
+   swap{1} 3 -1.
+
+   seq 2 0 : (0 <= valRep4 f{2} && valRep4 f{2} < p /\ t{1} = add_l4 f{2} _tt{2} 19 /\
+               0 <= valRep4 f{1} && valRep4 f{1} < p + 19 /\ _tt{2} = f{2}.[3]
+               /\ extracted_msbw{2} = W64.zerow
+               /\ tt0{2} = W64.of_int 19 /\ 19 <= valRep4 ff{2} && valRep4 ff{2} < p+19 /\
+               ff{2} = add_to_limb f{2} _tt{2} 19 /\
+               f{1}.[0] = add_l1 f{2} 19 /\ f{1}.[1] = add_l2 f{2} 19 /\
+               f{1}.[2] = add_l3 f{2} 19 /\ f{1}.[3] = ff.[3]{2}).
+   + auto => />. move => &1 &2 [#] H H0 H1 H2 H3 H4 H5 H6.
+   + rewrite valRep4_cmp //=.
+   + have !->: LEA_64 (add_l4 f{2} f{2}.[3] 19 + add_l4 f{2} f{2}.[3] 19) `>>` W8.one = add_l4 f{2} f{2}.[3] 19.
+   + rewrite helper_lemma_msb_is_not_set. move: H2. rewrite pVal.
+   + rewrite !valRep4E !/to_list !/val_digits !/mkseq -!iotaredE => />. move: W64.to_uint_cmp. smt().
+   + auto.
+   + move: H2. rewrite !valRep4E !pVal !/to_list !/val_digits !/mkseq -!iotaredE => />. smt().
+
+   seq 3 1 : (0 <= valRep4 f{2} && valRep4 f{2} < p /\
+               0 <= valRep4 f{1} && valRep4 f{1} < p + 19
+               /\ extracted_msbw{2} = W64.zerow /\ f{2} = f{2}
+               /\ tt0{2} = W64.of_int 19 /\ 19 <= valRep4 ff{2} && valRep4 ff{2} < p+19 /\
+               ff{2} = add_to_limb f{2} _tt{2} 19 /\ f{1}.[0] = add_l1 f{2} 19
+               /\ f{1}.[1] = add_l2 f{2} 19 /\
+               f{1}.[2] = add_l3 f{2} 19 /\ f{1}.[3] = ff.[3]{2} /\ f3{2} = W64.of_int 19 /\
+               t{1} = W64.of_int 19).
+   + ecall {2} (ph_to_19_by_invw). auto => />. move => &1 &2 [#] H H0 H1 H2 H3 H4 H5 H6 H7 H8.
+   + do split. smt(W64.to_uint_cmp). move: H0 limb4_ltP_cmp. smt(). move => H9 H10.
+   + rewrite helper_lemma_to_19.
+   + move: H2. rewrite pVal.
+   + rewrite !valRep4E !/to_list !/val_digits !/mkseq -!iotaredE => />. move: W64.to_uint_cmp. smt().
+   + auto.
+
+   ecall {2} (ph_subtraction ff{2} 19). auto => />.
+   + move => &1 &2 H H0 H1 H2 H3 H4 H5 H6 H7 H8. do split. move: H4. smt(pVal).
+   + move => H9 H10. rewrite H5 H6 H7 H8.
+   + rewrite !addcE !/carry_add !b2i0 => />.
+   + rewrite !subcE !/borrow_sub !b2i0 => />.
+   + rewrite !valRep4E !/to_list !/val_digits !/mkseq -!iotaredE => />.
+qed.
+
+
+
+
+
+
+
+
+
+
+
+
+
+
 lemma equiv_to_bytes_no_reduction:
-    equiv[M.__tobytes4 ~ ToBytesSpec.tobytes_no_reduction :
+    equiv[M.__tobytes4 ~ ToBytesSpec.to_bytes :
       f{1} = f{2} /\ 0 <= valRep4 f{1} < p
       ==>
       valRep4 res{1} = valRep4 res{2}
     ].
 proof.
     proc => />.
-    inline {2} 1. swap {2} 4 -1. swap{1} 9 -7.
-    seq 2 3: (#pre /\ t{1} = tt1{2} /\ tt1{2} = f0.[3]{2} /\ 0 <= valRep4 f0{2} < p /\ f0{2} = f{2}).
-    + wp; sp. ecall {2} (ph_remove_msb_if_set_lt_2_255 f0.[3]{2}). auto => />.
-    + move => &2 [#] H H0. do split. smt(W64.to_uint_cmp).
-    + move: H H0 upper_limb4_lt_2_255_range W64.to_uint_cmp pVal; 1:smt().
-    + move => H1 H2. rewrite helper_remove_msb_if_set /#.
+    swap {2} 2 -1. swap{1} 9 -7.
+    seq 2 1: (#pre /\ t{1} = _tt{2} /\ _tt{2} = f{2}.[3] /\ 0 <= valRep4 f{2} < p).
+    + ecall {2} (ph_msb_not_set f{2}.[3]). auto => />.
+    + move => &2 [#] H H0. do split.
+    + smt(W64.to_uint_cmp).
+    + move: H H0 limb4_lt_2_255_cmp W64.to_uint_cmp pVal; 1:smt().
+    + move => H1 H2. rewrite helper_lemma_msb_is_not_set /#.
 
-    seq 6 1 : (#pre /\ extracted_msbw0{2} = W64.zerow /\ aux_4{1} = extracted_msbw0{2}).
-    + auto => />.
-    + ecall {2} (ph_extract_msb_lt_2_255). auto => />.
-    + move => &2 H H0 H1 H2. do split. smt(W64.to_uint_cmp).
-    + move: H1 H2. rewrite valRep4E pE /to_list /val_digits /mkseq -iotaredE => />.
-    + smt(W64.to_uint_cmp). move => H3 H4.
-    + rewrite /SAR_64 /shift_mask /rflags_OF //= sarE /min => />.
-    + rewrite init_bits2w bits2wE -iotaredE /min //= upper_limb4_ltP_msbw.
-    + move: H H0. rewrite valRep4E pE /to_list /val_digits /mkseq -iotaredE => />.
-    + rewrite /W64.zerow of_intE bits2wE /int2bs /mkseq -iotaredE => />.
+    seq 6 1 : (#pre /\ extracted_msbw{2} = W64.zerow /\ aux_4{1} = extracted_msbw{2}).
+    + auto => />. ecall {2} (ph_extract_msb0). auto => />.
+    + move => &2 H H0. do split.
+    + smt(W64.to_uint_cmp).
+    + move: H H0 limb4_ltP_cmp. smt(). move => *.
+    + rewrite helper_lemma_extract_msb_0 /#.
 
-    seq 1 0 : (0 <= valRep4 f{1} && valRep4 f{1} < p - W64.to_uint (f.[3]{2}) /\ t{1} = tt1{2}
-               /\ tt1{2} = f0{2}.[3] /\
-               0 <= valRep4 f0{2} && valRep4 f0{2} < p /\ extracted_msbw0{2} = W64.zerow /\
-               aux_4{1} = extracted_msbw0{2} /\ f0{2} = f{2} /\
-               f{1} = Array4.of_list witness [f.[0]{2}; f.[1]{2}; f.[2]{2}; extracted_msbw0{2}]).
-    + auto => />. move => &2 H H0 H1 H2. do split.
-    + rewrite valRep4E /to_list /val_digits /mkseq -iotaredE => />. smt(W64.to_uint_cmp).
-    + move => H3. do split.
-    + move: H H0. rewrite !valRep4E !pE !/to_list !/val_digits !/mkseq -!iotaredE => />.
-    + rewrite to_uint0 => />. smt(W64.to_uint_cmp). apply Array4.ext_eq => i ib.
-    + rewrite !get_setE 1:/#.
-    + case (i = 3) => I. rewrite I => />.
-    + case (i = 2) => I0. rewrite I0 => />.
-    + case (i = 1) => I1. rewrite I1 => />.
-    + case (i = 0) => I2. rewrite I2 => />. rewrite get_out /#.
+    seq 1 0 : (0 <= valRep4 f{1} && valRep4 f{1} < p - W64.to_uint (f.[3]{2}) /\ t{1} = _tt{2}
+               /\ _tt{2} = f{2}.[3] /\
+               0 <= valRep4 f{2} && valRep4 f{2} < p /\ extracted_msbw{2} = W64.zerow /\
+               aux_4{1} = extracted_msbw{2} /\
+               f{1} = Array4.of_list witness [f.[0]{2}; f.[1]{2}; f.[2]{2}; extracted_msbw{2}]).
+    + auto => />. move => &2 H H0. do split.
+    + rewrite valRep4_cmp //=. move => H3. do split.
+    + rewrite valRep4_remove_limb4_ltP //=.
+    + rewrite valRep4_remove_limb4_ltP_structure //=.
 
-    seq 2 1 : (0 <= valRep4 f{1} && valRep4 f{1} < p - (W64.to_uint f.[3]{2}) + 19 * pow 2 196 /\
-               t{1} = tt1{2} /\ tt1{2} = f0{2}.[3] /\ 0 <= valRep4 f0{2} && valRep4 f0{2} < p
-               /\ extracted_msbw0{2} = W64.zerow /\ f0{2} = f{2}
-               /\ tt00{2} = W64.of_int 19 /\ f.[0]{1} = f.[0]{2} /\ f.[1]{1} = f.[1]{2} /\
-               f.[2]{1} = f.[2]{2} /\  f.[3]{1} = tt00{2}).
-   + ecall {2} (ph_to19). wp. auto => />. move => &2 [#] H H0 H1 H2. do split.
-   + move: H. rewrite !valRep4E !/to_list !/val_digits !/mkseq -!iotaredE => />.
-   + rewrite to_uint0 => />. smt(W64.to_uint_cmp). move => H3.
-   + have !->: W64.zerow `&` (of_int 19)%W64 + (of_int 19)%W64 = W64.of_int 19. smt(@W64).
-   + move: H0. rewrite !valRep4E pE !/to_list !/val_digits !/mkseq -!iotaredE => />. rewrite to_uint0 //=.
-   + smt(W64.to_uint_cmp).
+    seq 2 1 : (0 <= valRep4 f{1} && valRep4 f{1} < p - (W64.to_uint f.[3]{2}) + 19 * pow 2 192 /\
+               t{1} = _tt{2} /\ _tt{2} = f{2}.[3] /\ 0 <= valRep4 f{2} && valRep4 f{2} < p
+               /\ extracted_msbw{2} = W64.zerow /\
+               tt0{2} = W64.of_int 19 /\ f.[0]{1} = f.[0]{2} /\ f.[1]{1} = f.[1]{2} /\
+               f.[2]{1} = f.[2]{2} /\  f.[3]{1} = tt0{2} /\
+               f{1} = Array4.of_list witness [f.[0]{2}; f.[1]{2}; f.[2]{2}; tt0{2}]).
+   + ecall {2} (ph_to_19). auto => />. move => &2 [#] H H0 H1 H2.
+   + have E: W64.zerow `&` (of_int 19)%W64 + (of_int 19)%W64 = W64.of_int 19. smt(@W64).
+   + do split. rewrite valRep4_cmp //=. move => H3. do split.
+   + move: H H0. rewrite !valRep4E pE !/to_list !/val_digits !/mkseq -!iotaredE => />.
+   + rewrite E to_uint0 //=. smt(W64.to_uint_cmp).
+   + rewrite E. apply Array4.ext_eq => i ib. rewrite get_setE //=. smt(Array4.initE).
 
-   seq 0 0 : (#pre /\ f{1} = Array4.of_list witness [f.[0]{2}; f.[1]{2}; f.[2]{2}; tt00{2}]).
-   + skip. move => &1 &2 [#] H H0 H1 H2 H3 H4 H5 H6 H7 H8 H9 H10.
-   + auto => />. move => *. auto => />. rewrite -H8 -H9 -H10 H7.
-   + apply Array4.ext_eq => i ib.
-    + case (i = 3) => I. rewrite I => />.
-    + case (i = 2) => I0. rewrite I0 => />.
-    + case (i = 1) => I1. rewrite I1 => />.
-    + case (i = 0) => I2. rewrite I2 => />. rewrite get_out /#.
-
-    seq 10 1 : (0 <= valRep4 f0{2} && valRep4 f0{2} < p
-               /\ extracted_msbw0{2} = W64.zerow /\ f0{2} = f{2}
-               /\ tt00{2} = W64.of_int 19 /\ 19 <= valRep4 ff0{2} && valRep4 ff0{2} < p+19 /\
-               ff0{2} = add19 f0{2} /\ f{1}.[0] = add19_l1 f{2} /\ f{1}.[1] = add19_l2 f{2} /\
-               f{1}.[2] = add19_l3 f{2} /\ f{1}.[3] = W64.of_int 19 /\ t{1} = add19_l4 f0{2}
-               /\ t{1} = add19_l4 f{2}).
-   + ecall {2} (ph_addition19 f0{2}). auto => />. move => &1 [#] H H0 H1 H2 H3.
-   + do split. rewrite -H3 1:/#. move => H4.  rewrite -H3 1:/#.
-
-   seq 0 1 : (#pre /\ ff{2} = ff0{2}). auto => />.
+    seq 10 1 : (0 <= valRep4 f{2} && valRep4 f{2} < p
+               /\ extracted_msbw{2} = W64.zerow /\ _tt{2} = f{2}.[3]
+               /\ tt0{2} = W64.of_int 19 /\ 19 <= valRep4 ff{2} && valRep4 ff{2} < p+19 /\
+               ff{2} = (add_to_limb f{2} _tt{2} 19) /\ f{1}.[0] = add_l1 f{2} 19 /\
+               f{1}.[1] = add_l2 f{2} 19 /\ _tt{2} = f{2}.[3] /\
+               f{1}.[2] = add_l3 f{2} 19 /\ f{1}.[3] = W64.of_int 19  /\ t{1} = add_l4 f{2} _tt{2} 19).
+   + ecall {2} (ph_addition f{2} _tt{2} 19). auto => />. move => &1 [#] H H0 H1 H2.
+   + do split. move: H2. rewrite pVal 1:/#. move: limb4_ltP_cmp. move: H1 H2. smt().
+   move => H3 H4 H5. do split. rewrite -H5. move: valRep4_cmp. smt(). move => H6.
+   rewrite -H5 pVal. rewrite -valRep4_equiv_representation. move: H2. rewrite pVal 1:/#.
 
    swap{1} 3 -1.
-   seq 2 0 : (ff{2} = ff0{2} /\ 0 <= valRep4 f0{2} && valRep4 f0{2} < p /\ t{1} = add19_l4 f{2} /\
-               0 <= valRep4 f{1} && valRep4 f{1} < p + 19
-               /\ extracted_msbw0{2} = W64.zerow /\ f0{2} = f{2}
-               /\ tt00{2} = W64.of_int 19 /\ 19 <= valRep4 ff0{2} && valRep4 ff0{2} < p+19 /\
-               ff0{2} = add19 f0{2} /\ f{1}.[0] = add19_l1 f{2} /\ f{1}.[1] = add19_l2 f{2} /\
-               f{1}.[2] = add19_l3 f{2} /\ f{1}.[3] = ff0.[3]{2}).
-   + auto => />. move => &1 &2 [#] H H0 H1 H2 H3 H4 H5 H6. do split.
-   + rewrite valRep4E /to_list /val_digits /mkseq -iotaredE => />. smt(W64.to_uint_cmp). move => H7.
-   + do split. move: H2. rewrite !valRep4E !pVal !/to_list !/val_digits !/mkseq -!iotaredE => />.
-   + have ->: LEA_64 (add19_l4 f{2} + add19_l4 f{2}) `>>` W8.one = add19_l4 f{2}.
-   + rewrite helper_remove_msb_if_set. move: H0.
-   + rewrite !valRep4E !pVal !/to_list !/val_digits !/mkseq -!iotaredE => />.
-   + rewrite !addcE !/carry_add !b2i0 => />.
-   + case (18446744073709551616 <= u64i f{2}.[0] + 19 = false) => C. rewrite !C !b2i0 => />.
-   + have !->: 18446744073709551616 <= u64i f{2}.[1] = false. move: W64.to_uint_cmp. smt().
-   + have !->: 18446744073709551616 <= u64i f{2}.[2] = false. move: W64.to_uint_cmp. smt().
-   + rewrite !b2i0 => />. smt(W64.to_uint_cmp).
-   + move: C. rewrite not_false_to_true. move => C. rewrite !C !b2i1 => />.
-   + case (18446744073709551616 <= u64i f{2}.[1] + 1 = false) => C1. rewrite !C1 !b2i0 => />.
-   + have !->: 18446744073709551616 <= u64i f{2}.[2] = false. move: W64.to_uint_cmp. smt().
-   + rewrite !b2i0 => />. smt(W64.to_uint_cmp).
-   + move: C1. rewrite not_false_to_true. move => C1. rewrite !C1 !b2i1 => />.
-   + case (18446744073709551616 <= u64i f{2}.[2] + 1 = false) => C2. rewrite !C2 !b2i0 => />.
-   + smt(W64.to_uint_cmp).
-   + move: C2. rewrite not_false_to_true. move => C2. rewrite !C2 !b2i1 => />.
-   + rewrite !to_uintD of_uintK. smt(W64.to_uint_cmp).
-   + auto => />. move => H8. smt().
-   + have ->: LEA_64 (add19_l4 f{2} + add19_l4 f{2}) `>>` W8.one = add19_l4 f{2}.
-   + rewrite helper_remove_msb_if_set. move: H0.
-   + rewrite !valRep4E !pVal !/to_list !/val_digits !/mkseq -!iotaredE => />.
-   + rewrite !addcE !/carry_add !b2i0 => />.
-   + case (18446744073709551616 <= u64i f{2}.[0] + 19 = false) => C. rewrite !C !b2i0 => />.
-   + have !->: 18446744073709551616 <= u64i f{2}.[1] = false. move: W64.to_uint_cmp. smt().
-   + have !->: 18446744073709551616 <= u64i f{2}.[2] = false. move: W64.to_uint_cmp. smt().
-   + rewrite !b2i0 => />. smt(W64.to_uint_cmp).
-   + move: C. rewrite not_false_to_true. move => C. rewrite !C !b2i1 => />.
-   + case (18446744073709551616 <= u64i f{2}.[1] + 1 = false) => C1. rewrite !C1 !b2i0 => />.
-   + have !->: 18446744073709551616 <= u64i f{2}.[2] = false. move: W64.to_uint_cmp. smt().
-   + rewrite !b2i0 => />. smt(W64.to_uint_cmp).
-   + move: C1. rewrite not_false_to_true. move => C1. rewrite !C1 !b2i1 => />.
-   + case (18446744073709551616 <= u64i f{2}.[2] + 1 = false) => C2. rewrite !C2 !b2i0 => />.
-   + smt(W64.to_uint_cmp).
-   + move: C2. rewrite not_false_to_true. move => C2. rewrite !C2 !b2i1 => />.
-   + rewrite !to_uintD of_uintK. smt(W64.to_uint_cmp). auto => />. auto => />.
 
-   seq 3 1 : (ff{2} = ff0{2} /\ 0 <= valRep4 f0{2} && valRep4 f0{2} < p /\
+   seq 2 0 : (0 <= valRep4 f{2} && valRep4 f{2} < p /\ t{1} = add_l4 f{2} _tt{2} 19 /\
+               0 <= valRep4 f{1} && valRep4 f{1} < p + 19 /\ _tt{2} = f{2}.[3]
+               /\ extracted_msbw{2} = W64.zerow
+               /\ tt0{2} = W64.of_int 19 /\ 19 <= valRep4 ff{2} && valRep4 ff{2} < p+19 /\
+               ff{2} = add_to_limb f{2} _tt{2} 19 /\
+               f{1}.[0] = add_l1 f{2} 19 /\ f{1}.[1] = add_l2 f{2} 19 /\
+               f{1}.[2] = add_l3 f{2} 19 /\ f{1}.[3] = ff.[3]{2}).
+   + auto => />. move => &1 &2 [#] H H0 H1 H2 H3 H4 H5 H6.
+   + rewrite valRep4_cmp //=.
+   + have !->: LEA_64 (add_l4 f{2} f{2}.[3] 19 + add_l4 f{2} f{2}.[3] 19) `>>` W8.one = add_l4 f{2} f{2}.[3] 19.
+   + rewrite helper_lemma_msb_is_not_set. move: H2. rewrite pVal.
+   + rewrite !valRep4E !/to_list !/val_digits !/mkseq -!iotaredE => />. move: W64.to_uint_cmp. smt().
+   + auto.
+   + move: H2. rewrite !valRep4E !pVal !/to_list !/val_digits !/mkseq -!iotaredE => />. smt().
+
+   seq 3 1 : (0 <= valRep4 f{2} && valRep4 f{2} < p /\
                0 <= valRep4 f{1} && valRep4 f{1} < p + 19
-               /\ extracted_msbw0{2} = W64.zerow /\ f0{2} = f{2}
-               /\ tt00{2} = W64.of_int 19 /\ 19 <= valRep4 ff0{2} && valRep4 ff0{2} < p+19 /\
-               ff0{2} = add19 f0{2} /\ f{1}.[0] = add19_l1 f{2} /\ f{1}.[1] = add19_l2 f{2} /\
-               f{1}.[2] = add19_l3 f{2} /\ f{1}.[3] = ff0.[3]{2} /\ f3{2} = W64.of_int 19 /\
+               /\ extracted_msbw{2} = W64.zerow /\ f{2} = f{2}
+               /\ tt0{2} = W64.of_int 19 /\ 19 <= valRep4 ff{2} && valRep4 ff{2} < p+19 /\
+               ff{2} = add_to_limb f{2} _tt{2} 19 /\ f{1}.[0] = add_l1 f{2} 19
+               /\ f{1}.[1] = add_l2 f{2} 19 /\
+               f{1}.[2] = add_l3 f{2} 19 /\ f{1}.[3] = ff.[3]{2} /\ f3{2} = W64.of_int 19 /\
                t{1} = W64.of_int 19).
-   + ecall {2} (ph_sar_inv_t). auto => />. move => &1 &2 [#] H H0 H1 H2 H3 H4 H5 H6 H7 H8.
-   + do split. smt(W64.to_uint_cmp). move: H4.
-   + rewrite !valRep4E !pVal !/to_list !/val_digits !/mkseq -!iotaredE => />.
-   + rewrite !addcE !/carry_add !b2i0 => />.
-   + case (18446744073709551616 <= u64i f{2}.[0] + 19 = false) => C. rewrite !C !b2i0 => />.
-   + have !->: 18446744073709551616 <= u64i f{2}.[1] = false. move: W64.to_uint_cmp. smt().
-   + have !->: 18446744073709551616 <= u64i f{2}.[2] = false. move: W64.to_uint_cmp. smt().
-   + rewrite !b2i0 => />. smt(W64.to_uint_cmp).
-   + move: C. rewrite not_false_to_true. move => C. rewrite !C !b2i1 => />.
-   + case (18446744073709551616 <= u64i f{2}.[1] + 1 = false) => C1. rewrite !C1 !b2i0 => />.
-   + have !->: 18446744073709551616 <= u64i f{2}.[2] = false. move: W64.to_uint_cmp. smt().
-   + rewrite !b2i0 => />. smt(W64.to_uint_cmp).
-   + move: C1. rewrite not_false_to_true. move => C1. rewrite !C1 !b2i1 => />.
-   + case (18446744073709551616 <= u64i f{2}.[2] + 1 = false) => C2. rewrite !C2 !b2i0 => />.
-   + smt(W64.to_uint_cmp).
-   + move: C2. rewrite not_false_to_true. move => C2. rewrite !C2 !b2i1 => />.
-   + rewrite !to_uintD of_uintK. smt(W64.to_uint_cmp).
-   + auto => />. move => H9 H10.
-   + rewrite helper_sar_inv_t 1:/#. auto.
-   ecall {2} (ph_subtraction19 ff{2}). auto => />.
-   + move => &1 &2 H H0 H1 H2 H3 H4 H5 H6 H7 H8. do split.
-   + move: H4. rewrite !valRep4E !pVal !/to_list !/val_digits !/mkseq -!iotaredE => />.
-   + rewrite !addcE !/carry_add !b2i0 => />.
-   + case (18446744073709551616 <= u64i f{2}.[0] + 19 = false) => C. rewrite !C !b2i0 => />.
-   + have !->: 18446744073709551616 <= u64i f{2}.[1] = false. move: W64.to_uint_cmp. smt().
-   + have !->: 18446744073709551616 <= u64i f{2}.[2] = false. move: W64.to_uint_cmp. smt().
-   + rewrite !b2i0 => />. smt(W64.to_uint_cmp).
-   + move: C. rewrite not_false_to_true. move => C. rewrite !C !b2i1 => />.
-   + case (18446744073709551616 <= u64i f{2}.[1] + 1 = false) => C1. rewrite !C1 !b2i0 => />.
-   + have !->: 18446744073709551616 <= u64i f{2}.[2] = false. move: W64.to_uint_cmp. smt().
-   + rewrite !b2i0 => />. smt(W64.to_uint_cmp).
-   + move: C1. rewrite not_false_to_true. move => C1. rewrite !C1 !b2i1 => />.
-   + case (18446744073709551616 <= u64i f{2}.[2] + 1 = false) => C2. rewrite !C2 !b2i0 => />.
-   + smt(W64.to_uint_cmp).
-   + move: C2. rewrite not_false_to_true. move => C2. rewrite !C2 !b2i1 => />.
-   + rewrite !to_uintD of_uintK. smt(W64.to_uint_cmp).
-   + move => H9 H10 H11. rewrite -H11 H5 H6 H7 H8.
+   + ecall {2} (ph_to_19_by_invw). auto => />. move => &1 &2 [#] H H0 H1 H2 H3 H4 H5 H6 H7 H8.
+   + do split. smt(W64.to_uint_cmp). move: H0 limb4_ltP_cmp. smt(). move => H9 H10.
+   + rewrite helper_lemma_to_19.
+   + move: H2. rewrite pVal.
+   + rewrite !valRep4E !/to_list !/val_digits !/mkseq -!iotaredE => />. move: W64.to_uint_cmp. smt().
+   + auto.
+
+   ecall {2} (ph_subtraction ff{2} 19). auto => />.
+   + move => &1 &2 H H0 H1 H2 H3 H4 H5 H6 H7 H8. do split. move: H4. smt(pVal).
+   + move => H9 H10. rewrite H5 H6 H7 H8.
    + rewrite !addcE !/carry_add !b2i0 => />.
    + rewrite !subcE !/borrow_sub !b2i0 => />.
    + rewrite !valRep4E !/to_list !/val_digits !/mkseq -!iotaredE => />.
-   + rewrite !mulzDr -!mulzA !to_uintD !to_uintN (modz_small 19 (pow 2 64)) 1:/# => />.
-   + rewrite !of_uintK => />.
-   + case (18446744073709551616 <= u64i f{2}.[0] + 19 = false) => C. rewrite !C !b2i0 => />.
-   + have ->: (18446744073709551616 <= u64i f{2}.[1] = false). move: W64.to_uint_cmp => />. smt().
-   + have ->: (18446744073709551616 <= u64i f{2}.[2] = false). move: W64.to_uint_cmp => />. smt().
-   + rewrite (pmod_small (u64i f{2}.[3]) 18446744073709551616). move: W64.to_uint_cmp => />. smt().
-   + rewrite (pmod_small (u64i f{2}.[2]) 18446744073709551616). move: W64.to_uint_cmp => />. smt().
-   + rewrite (pmod_small (u64i f{2}.[1]) 18446744073709551616). move: W64.to_uint_cmp => />. smt().
-   + rewrite (pmod_small (u64i f{2}.[0] + 19) 18446744073709551616). move: W64.to_uint_cmp => />. smt().
-   + have ->: u64i f{2}.[0] + 19 < 19 = false. move: W64.to_uint_cmp => />. smt().
-   + have ->: u64i f{2}.[1] < 0 = false. move: W64.to_uint_cmp => />. smt().
-   + have ->: u64i f{2}.[2] < 0 = false. move: W64.to_uint_cmp => />. smt().
-   + rewrite !b2i0 => />.
-   + rewrite (pmod_small (u64i f{2}.[3]) 18446744073709551616). move: W64.to_uint_cmp => />. smt().
-   + rewrite (pmod_small (u64i f{2}.[2]) 18446744073709551616). move: W64.to_uint_cmp => />. smt().
-   + rewrite (pmod_small (u64i f{2}.[1]) 18446744073709551616). move: W64.to_uint_cmp => />. smt().
-   + have ->: (u64i f{2}.[0] + 18446744073709551616) %% 18446744073709551616 = (u64i f{2}.[0] + 18446744073709551616) - 18446744073709551616. move: W64.to_uint_cmp. smt().
-   + ring.
-
-   move: C. rewrite not_false_to_true. move => C. rewrite !C !b2i1.
-   case(18446744073709551616 <= u64i f{2}.[1] + 1 = false) => C1. rewrite !C1 !b2i0 => />.
-   + have ->: (18446744073709551616 <= u64i f{2}.[2] = false). move: W64.to_uint_cmp => />. smt().
-   + rewrite (pmod_small (u64i f{2}.[3]) 18446744073709551616). move: W64.to_uint_cmp => />. smt().
-   + rewrite (pmod_small (u64i f{2}.[2]) 18446744073709551616). move: W64.to_uint_cmp => />. smt().
-   + have ->: ((u64i f{2}.[0] + 19) %% 18446744073709551616 < 19) = true. move: W64.to_uint_cmp => />. smt().
-   + have ->: ((u64i f{2}.[1] + 1) %% 18446744073709551616 < 1) = false. move: W64.to_uint_cmp => />. smt().
-   + have ->: ((u64i f{2}.[2] < 0)) = false. move: W64.to_uint_cmp => />. smt().
-   + rewrite !b2i0 !b2i1 => />.
-   + rewrite (pmod_small (u64i f{2}.[3]) 18446744073709551616). move: W64.to_uint_cmp => />. smt().
-   + rewrite (pmod_small (u64i f{2}.[2]) 18446744073709551616). move: W64.to_uint_cmp => />. smt().
-   + have ->: (u64i f{2}.[0] + 19) %% 18446744073709551616 = (u64i f{2}.[0] + 19) - 18446744073709551616. move: W64.to_uint_cmp => />. smt().
-   + rewrite (pmod_small (u64i f{2}.[1] + 1) 18446744073709551616). move: W64.to_uint_cmp => />. smt().
-   + have ->: (u64i f{2}.[1] + 1 + 18446744073709551615) %% 18446744073709551616 = (u64i f{2}.[1] + 1 + 18446744073709551615) - 18446744073709551616. move: W64.to_uint_cmp => />. smt(). auto => />.
-   + rewrite (pmod_small (u64i f{2}.[0]) 18446744073709551616). move: W64.to_uint_cmp => />. smt().
-   + ring.
-
-   move: C1. rewrite not_false_to_true. move => C1. rewrite !C1 !b2i1.
-   case(18446744073709551616 <= u64i f{2}.[2] + 1 = false) => C2. rewrite !C2 !b2i0 => />.
-   + rewrite (pmod_small (u64i f{2}.[3]) 18446744073709551616). move: W64.to_uint_cmp => />. smt().
-   + have ->: ((u64i f{2}.[0] + 19) %% 18446744073709551616 < 19) = true. move: W64.to_uint_cmp => />. smt().
-   + have ->: ((u64i f{2}.[1] + 1) %% 18446744073709551616 < 1) = true. move: W64.to_uint_cmp => />. smt().
-   + rewrite  !b2i1 => />.
-   + have ->: (u64i f{2}.[0] + 19) %% 18446744073709551616 = (u64i f{2}.[0] + 19) - 18446744073709551616. move: W64.to_uint_cmp => />. smt().
-   + have ->: (u64i f{2}.[2] + 1) %% 18446744073709551616 < 1 = false. move: W64.to_uint_cmp => />. smt().
-   + rewrite (pmod_small (u64i f{2}.[0]) 18446744073709551616). move: W64.to_uint_cmp => />. smt().
-   + rewrite (pmod_small (u64i f{2}.[2] + 1) 18446744073709551616). move: W64.to_uint_cmp => />. smt().
-   + have ->: (u64i f{2}.[2] + 1 + 18446744073709551615) %% 18446744073709551616 = (u64i f{2}.[2] + 1 + 18446744073709551615) - 18446744073709551616. move: W64.to_uint_cmp => />. smt(). auto => />.
-   + have ->: (u64i f{2}.[1] + 1) %% 18446744073709551616 = (u64i f{2}.[1] + 1 - 18446744073709551616). move: W64.to_uint_cmp => />. smt(). rewrite !b2i0 => />.
-   + rewrite (pmod_small (u64i f{2}.[3]) 18446744073709551616). move: W64.to_uint_cmp => />. smt().
-   + rewrite (pmod_small (u64i f{2}.[1]) 18446744073709551616). move: W64.to_uint_cmp => />. smt().
-   + ring.
-
-   move: C2. rewrite not_false_to_true. move => C2. rewrite !C2 !b2i1.
-   have E: (18446744073709551616 <= u64i f{2}.[3] + 1 = false).
-   + move: (W64.to_uint_cmp f{2}.[3])  (upper_limb4_ltP_range f{2}) H H0 H1 H2 H3 H4 H9.
-   + rewrite !valRep4E !pE !/to_list !/val_digits !/mkseq -!iotaredE => />.
-   + rewrite !mulzDr -!mulzA   (modz_small 0 (pow 2 64)) 1:/# => />; 1:smt().
-
-   + have ->: ((u64i f{2}.[0] + 19) %% 18446744073709551616 < 19) = true. move: W64.to_uint_cmp => />. smt().
-   + have ->: ((u64i f{2}.[1] + 1) %% 18446744073709551616 < 1) = true. move: W64.to_uint_cmp => />. smt().
-   + rewrite  !b2i1 => />.
-   + have !->: (u64i f{2}.[0] + 19) %% 18446744073709551616 = (u64i f{2}.[0] + 19) - 18446744073709551616. move: W64.to_uint_cmp => />. smt().
-   + have ->: (u64i f{2}.[2] + 1) %% 18446744073709551616 < 1 = true. move: W64.to_uint_cmp => />. smt().
-   + rewrite (pmod_small (u64i f{2}.[0]) 18446744073709551616). move: W64.to_uint_cmp => />. smt().
-   + have !->: (u64i f{2}.[2] + 1) %% 18446744073709551616 = (u64i f{2}.[2] + 1) - 18446744073709551616. move: W64.to_uint_cmp => />. smt(). auto => />.
-   + have !->: (u64i f{2}.[1] + 1) %% 18446744073709551616 = (u64i f{2}.[1] + 1) - 18446744073709551616. move: W64.to_uint_cmp => />. smt(). auto => />.
-   + rewrite pmod_small. move: W64.to_uint_cmp => />. smt().
-   + rewrite pmod_small. move: W64.to_uint_cmp => />. smt().
-   + rewrite !b2i1 => />.
-   + rewrite (pmod_small (u64i f{2}.[3] + 1) 18446744073709551616). move: W64.to_uint_cmp => />. smt().
-   + have !->: (u64i f{2}.[3] + 1 + 18446744073709551615) %% 18446744073709551616 = (u64i f{2}.[3] + 1 + 18446744073709551615) - 18446744073709551616. move: W64.to_uint_cmp => />. smt().
-   + ring.
-qed.
-
-(** Case p <= valRep4 < 2*p (some lemmas extend to 2**256)**)
-
-lemma h_sar_inv_t_of:
-  hoare [ToBytesSpec.sar_inv_t :
-      pow 2 63 <= W64.to_uint t < W64.modulus
-      ==>
-      res = W64.zerow].
-    proc => />. auto => />.
-    move => &hr H H0.
-    have ->: (SAR_64 t{hr} ((of_int 63))%W8).`6 = W64.onew.
-    + rewrite /SAR_64 /shift_mask /rflags_OF //= sarE /min => />.
-    rewrite init_bits2w bits2wE -iotaredE /min //= upper_limb4_geqP_msbw.
-    move: H upper_limb4_geq_2_255_range W64.to_uint_cmp; 1:smt().
-    + rewrite /W64.onew of_intE bits2wE /int2bs /mkseq -iotaredE => />.
-    have ->: invw W64.onew = W64.zerow.
-    + rewrite /invw mapE /W64.zerow /W64.zero bits2wE /int2bs /mkseq -iotaredE => />.
-    + rewrite wordP => i ib. rewrite !initiE 1,2,3:/# //=.
-    rewrite wordP => i ib.
-    rewrite /W64.zerow /W64.zero !bits2wE !/int2bs !/mkseq -!iotaredE => />.
-    rewrite !initiE 1,2:/# //= /#.
-qed.
-
-lemma ph_sar_inv_t_of:
-  phoare [ToBytesSpec.sar_inv_t :
-      pow 2 63 <= W64.to_uint t < W64.modulus
-      ==>
-      res = W64.zerow] = 1%r.
-proof.
-    by conseq ill_sar_inv_t (h_sar_inv_t_of).
-qed.
-
-(** Subtraction **)
-
-lemma h_subtraction0 (r: Rep4):
-  hoare [ToBytesSpec.subtraction :
-      r = f /\ operand2 = W64.of_int 0
-      ==>
-      valRep4 r = valRep4 res
-  ].
-proof.
-    proc. auto => />. move => &hr.
-    rewrite !subcE !/borrow_sub !b2i0 => />.
-    rewrite !valRep4E !/to_list !/val_digits !/mkseq -!iotaredE => />.
-    rewrite !mulzDr -!mulzA !to_uintD !to_uintN (modz_small 0 (pow 2 64)) 1:/# => />.
-    have ->: u64i r.[0] < 0 = false. move: W64.to_uint_cmp; 1:smt().
-    have ->: u64i r.[1] < 0 = false. move: W64.to_uint_cmp; 1:smt().
-    have ->: u64i r.[2] < 0 = false. move: W64.to_uint_cmp; 1:smt().
-    rewrite pmod_small. move: W64.to_uint_cmp; 1:smt().
-    rewrite !b2i0 => />.
-    rewrite pmod_small. move: W64.to_uint_cmp; 1:smt().
-    rewrite pmod_small. move: W64.to_uint_cmp; 1:smt().
-    rewrite pmod_small. move: W64.to_uint_cmp; 1:smt().
-    auto.
-qed.
-
-lemma ph_subtraction0 (r: Rep4):
-  phoare [ToBytesSpec.subtraction :
-      r = f /\ operand2 = W64.of_int 0
-      ==>
-      valRep4 r = valRep4 res
-  ] = 1%r.
-proof.
-    by conseq ill_subtraction (h_subtraction0 r).
 qed.
